riscv proofs: update for generic maxIRQ
Use properties from Arch_Kernel_Config_Lemmas instead of unfolding,
which also simplifies most proofs that used these Kernel_Config
constants.

Improve the pspace_distinct' proof in the infoflow refine state example
by making use of the new Sorted_Addresses library.

Signed-off-by: Gerwin Klein <gerwin.klein@proofcraft.systems>

proof/infoflow/refine/RISCV64/Example_Valid_StateH.thy
@@ -54,8 +54,8 @@ definition Low_cte' :: "10 word \<Rightarrow> cte option" where
 
 definition Low_cte :: "obj_ref \<Rightarrow> obj_ref \<Rightarrow> kernel_object option" where
   "Low_cte \<equiv> \<lambda>base offs.
-     if is_aligned offs 5 \<and> base \<le> offs \<and> offs \<le> base + 2 ^ 15 - 1
-     then map_option (\<lambda>cte. KOCTE cte) (Low_cte' (ucast (offs - base >> 5)))
+     if is_aligned offs cte_level_bits \<and> base \<le> offs \<and> offs \<le> base + 2 ^ 15 - 1
+     then map_option (\<lambda>cte. KOCTE cte) (Low_cte' (ucast (offs - base >> cte_level_bits)))
      else None"
 
 
@@ -88,8 +88,8 @@ definition High_cte' :: "10 word \<Rightarrow> cte option" where
 
 definition High_cte :: "obj_ref \<Rightarrow> obj_ref \<Rightarrow> kernel_object option" where
   "High_cte \<equiv> \<lambda>base offs.
-     if is_aligned offs 5 \<and> base \<le> offs \<and> offs \<le> base + 2 ^ 15 - 1
-     then map_option (\<lambda>cte. KOCTE cte) (High_cte' (ucast (offs - base >> 5)))
+     if is_aligned offs cte_level_bits \<and> base \<le> offs \<and> offs \<le> base + 2 ^ 15 - 1
+     then map_option (\<lambda>cte. KOCTE cte) (High_cte' (ucast (offs - base >> cte_level_bits)))
      else None"
 
 
@@ -113,8 +113,8 @@ definition Silc_cte' :: "10 word \<Rightarrow> cte option" where
 
 definition Silc_cte :: "obj_ref \<Rightarrow> obj_ref \<Rightarrow> kernel_object option" where
   "Silc_cte \<equiv> \<lambda>base offs.
-     if is_aligned offs 5 \<and> base \<le> offs \<and> offs \<le> base + 2 ^ 15 - 1
-     then map_option (\<lambda>cte. KOCTE cte) (Silc_cte' (ucast (offs - base >> 5)))
+     if is_aligned offs cte_level_bits \<and> base \<le> offs \<and> offs \<le> base + 2 ^ 15 - 1
+     then map_option (\<lambda>cte. KOCTE cte) (Silc_cte' (ucast (offs - base >> cte_level_bits)))
      else None"
 
 
@@ -309,13 +309,12 @@ definition option_update_range :: "('a \<Rightarrow> 'b option) \<Rightarrow> ('
   "option_update_range f g \<equiv> \<lambda>x. case f x of None \<Rightarrow> g x | Some y \<Rightarrow> Some y"
 
 definition kh0H :: "(obj_ref \<rightharpoonup> kernel_object)" where
-  "kh0H \<equiv> (option_update_range (\<lambda>x. if \<exists>irq :: irq. init_irq_node_ptr + (ucast irq << 5) = x
-                                     then Some (KOCTE (CTE NullCap Null_mdb)) else None) \<circ>
+  "kh0H \<equiv> (option_update_range (\<lambda>x. if \<exists>irq :: irq. init_irq_node_ptr + (ucast irq << cte_level_bits) = x
+                                     then Some (KOCTE irq_cte) else None) \<circ>
            option_update_range (Low_cte Low_cnode_ptr) \<circ>
            option_update_range (High_cte High_cnode_ptr) \<circ>
            option_update_range (Silc_cte Silc_cnode_ptr) \<circ>
            option_update_range [ntfn_ptr \<mapsto> KONotification ntfnH] \<circ>
-           option_update_range [irq_cnode_ptr \<mapsto> KOCTE irq_cte] \<circ>
            option_update_range (Low_pdH Low_pd_ptr) \<circ>
            option_update_range (High_pdH High_pd_ptr) \<circ>
            option_update_range (Low_ptH Low_pt_ptr) \<circ>
@@ -344,10 +343,9 @@ lemma s0_ptrs_aligned:
   "is_aligned idle_tcb_ptr 10"
   "is_aligned ntfn_ptr 5"
   "is_aligned shared_page_ptr_virt 21"
-  "is_aligned irq_cnode_ptr 10"
   "is_aligned Low_pool_ptr 12"
   "is_aligned High_pool_ptr 12"
-  by (simp add: is_aligned_def s0_ptr_defs)+
+  by (simp add: is_aligned_def s0_ptr_defs irq_len_val cte_level_bits_def)+
 
 
 text \<open>Page offset lemmas\<close>
@@ -620,14 +618,15 @@ lemma cnode_offs_max:
 
 definition cnode_offs_range where
   "cnode_offs_range (ptr :: obj_ref) \<equiv> {x. ptr \<le> x \<and> x \<le> ptr + 2 ^ 15 - 1}
-                                     \<inter> {x. is_aligned x 5}"
+                                     \<inter> {x. is_aligned x cte_level_bits}"
 
 lemma cnode_offs_in_range':
   "\<lbrakk> is_aligned ptr 15; length x = 10 \<rbrakk> \<Longrightarrow> ptr + of_bl x * 0x20 \<in> cnode_offs_range ptr"
   apply (simp add: cnode_offs_min' cnode_offs_max' cnode_offs_range_def add.commute)
   apply (rule is_aligned_add)
    apply (erule is_aligned_weaken)
-   apply simp
+   apply (simp add: cte_level_bits_def)
+  apply (simp add: cte_level_bits_def)
   apply (rule_tac is_aligned_mult_triv2[where x="of_bl x" and n=5, simplified])
   done
 
@@ -637,15 +636,15 @@ lemma cnode_offs_in_range:
   "length x = 10 \<Longrightarrow> Silc_cnode_ptr + of_bl x * 0x20 \<in> cnode_offs_range Silc_cnode_ptr"
   by (simp_all add: cnode_offs_in_range' s0_ptrs_aligned)
 
-lemma le_mask_eq:
+lemma le_mask_eq: (* FIXME: move to WordLib or eliminate *)
   "x \<le> 2 ^ n - 1 \<Longrightarrow> x AND mask n = (x :: 'a :: len word)"
   apply (unfold word_less_alt word_numeral_alt)
   apply (simp add: word_of_int_power_hom mask_eq_exp_minus_1[symmetric])
   apply (erule word_le_mask_eq)
   done
 
-lemma word_div_mult':
-  fixes c :: obj_ref
+lemma word_div_mult': (* FIXME: move to WordLib or eliminate *)
+  fixes c :: "'a :: len word"
   shows "\<lbrakk> 0 < c; a \<le> b * c \<rbrakk> \<Longrightarrow> a div c \<le> b"
   apply (simp add: word_le_nat_alt unat_div)
   apply (simp add: less_Suc_eq_le[symmetric])
@@ -671,7 +670,7 @@ lemma cnode_offs_range_correct':
    apply simp
    apply (rule word_diff_ls')
     apply (drule_tac a=x and n=5 in aligned_le_sharp)
-     apply simp
+     apply (simp add: cte_level_bits_def)
     apply (simp add: add.commute)
     apply (subst(asm) mask_out_add_aligned[symmetric])
      apply (erule is_aligned_weaken)
@@ -681,7 +680,7 @@ lemma cnode_offs_range_correct':
   apply (clarsimp simp: neg_mask_is_div[where n=5, simplified, symmetric])
   apply (subst is_aligned_neg_mask_eq)
    apply (rule aligned_sub_aligned)
-     apply assumption
+     apply (simp add: cte_level_bits_def)
     apply (erule is_aligned_weaken)
     apply simp
    apply simp
@@ -819,81 +818,81 @@ lemma kh0H_dom_distinct:
   "Low_tcb_ptr \<notin> cnode_offs_range Silc_cnode_ptr"
   "High_pool_ptr \<notin> cnode_offs_range Silc_cnode_ptr"
   "Low_pool_ptr \<notin> cnode_offs_range Silc_cnode_ptr"
-  "irq_cnode_ptr \<notin> cnode_offs_range Silc_cnode_ptr"
+  "init_irq_node_ptr \<notin> cnode_offs_range Silc_cnode_ptr"
   "ntfn_ptr \<notin> cnode_offs_range Silc_cnode_ptr"
   "idle_tcb_ptr \<notin> cnode_offs_range Low_cnode_ptr"
   "High_tcb_ptr \<notin> cnode_offs_range Low_cnode_ptr"
   "Low_tcb_ptr \<notin> cnode_offs_range Low_cnode_ptr"
   "High_pool_ptr \<notin> cnode_offs_range Low_cnode_ptr"
   "Low_pool_ptr \<notin> cnode_offs_range Low_cnode_ptr"
-  "irq_cnode_ptr \<notin> cnode_offs_range Low_cnode_ptr"
+  "init_irq_node_ptr \<notin> cnode_offs_range Low_cnode_ptr"
   "ntfn_ptr \<notin> cnode_offs_range Low_cnode_ptr"
   "idle_tcb_ptr \<notin> cnode_offs_range High_cnode_ptr"
   "High_tcb_ptr \<notin> cnode_offs_range High_cnode_ptr"
   "Low_tcb_ptr \<notin> cnode_offs_range High_cnode_ptr"
   "High_pool_ptr \<notin> cnode_offs_range High_cnode_ptr"
   "Low_pool_ptr \<notin> cnode_offs_range High_cnode_ptr"
-  "irq_cnode_ptr \<notin> cnode_offs_range High_cnode_ptr"
+  "init_irq_node_ptr \<notin> cnode_offs_range High_cnode_ptr"
   "ntfn_ptr \<notin> cnode_offs_range High_cnode_ptr"
   "idle_tcb_ptr \<notin> pt_offs_range Low_pd_ptr"
   "High_tcb_ptr \<notin> pt_offs_range Low_pd_ptr"
   "Low_tcb_ptr \<notin> pt_offs_range Low_pd_ptr"
   "High_pool_ptr \<notin> pt_offs_range Low_pd_ptr"
   "Low_pool_ptr \<notin> pt_offs_range Low_pd_ptr"
-  "irq_cnode_ptr \<notin> pt_offs_range Low_pd_ptr"
+  "init_irq_node_ptr \<notin> pt_offs_range Low_pd_ptr"
   "ntfn_ptr \<notin> pt_offs_range Low_pd_ptr"
   "idle_tcb_ptr \<notin> pt_offs_range High_pd_ptr"
   "High_tcb_ptr \<notin> pt_offs_range High_pd_ptr"
   "Low_tcb_ptr \<notin> pt_offs_range High_pd_ptr"
   "High_pool_ptr \<notin> pt_offs_range High_pd_ptr"
   "Low_pool_ptr \<notin> pt_offs_range High_pd_ptr"
-  "irq_cnode_ptr \<notin> pt_offs_range High_pd_ptr"
+  "init_irq_node_ptr \<notin> pt_offs_range High_pd_ptr"
   "ntfn_ptr \<notin> pt_offs_range High_pd_ptr"
   "idle_tcb_ptr \<notin> pt_offs_range riscv_global_pt_ptr"
   "High_tcb_ptr \<notin> pt_offs_range riscv_global_pt_ptr"
   "Low_tcb_ptr \<notin> pt_offs_range riscv_global_pt_ptr"
   "High_pool_ptr \<notin> pt_offs_range riscv_global_pt_ptr"
   "Low_pool_ptr \<notin> pt_offs_range riscv_global_pt_ptr"
-  "irq_cnode_ptr \<notin> pt_offs_range riscv_global_pt_ptr"
+  "init_irq_node_ptr \<notin> pt_offs_range riscv_global_pt_ptr"
   "ntfn_ptr \<notin> pt_offs_range riscv_global_pt_ptr"
   "idle_tcb_ptr \<notin> pt_offs_range Low_pt_ptr"
   "High_tcb_ptr \<notin> pt_offs_range Low_pt_ptr"
   "Low_tcb_ptr \<notin> pt_offs_range Low_pt_ptr"
   "High_pool_ptr \<notin> pt_offs_range Low_pt_ptr"
   "Low_pool_ptr \<notin> pt_offs_range Low_pt_ptr"
-  "irq_cnode_ptr \<notin> pt_offs_range Low_pt_ptr"
+  "init_irq_node_ptr \<notin> pt_offs_range Low_pt_ptr"
   "ntfn_ptr \<notin> pt_offs_range Low_pt_ptr"
   "idle_tcb_ptr \<notin> pt_offs_range High_pt_ptr"
   "High_tcb_ptr \<notin> pt_offs_range High_pt_ptr"
   "Low_tcb_ptr \<notin> pt_offs_range High_pt_ptr"
   "High_pool_ptr \<notin> pt_offs_range High_pt_ptr"
   "Low_pool_ptr \<notin> pt_offs_range High_pt_ptr"
-  "irq_cnode_ptr \<notin> pt_offs_range High_pt_ptr"
+  "init_irq_node_ptr \<notin> pt_offs_range High_pt_ptr"
   "ntfn_ptr \<notin> pt_offs_range High_pt_ptr"
   "idle_tcb_ptr \<notin> tcb_offs_range Low_tcb_ptr"
   "High_tcb_ptr \<notin> tcb_offs_range Low_tcb_ptr"
   "High_pool_ptr \<notin> tcb_offs_range Low_tcb_ptr"
   "Low_pool_ptr \<notin> tcb_offs_range Low_tcb_ptr"
-  "irq_cnode_ptr \<notin> tcb_offs_range Low_tcb_ptr"
+  "init_irq_node_ptr \<notin> tcb_offs_range Low_tcb_ptr"
   "ntfn_ptr \<notin> tcb_offs_range Low_tcb_ptr"
   "idle_tcb_ptr \<notin> tcb_offs_range High_tcb_ptr"
   "Low_tcb_ptr \<notin> tcb_offs_range High_tcb_ptr"
   "High_pool_ptr \<notin> tcb_offs_range High_tcb_ptr"
   "Low_pool_ptr \<notin> tcb_offs_range High_tcb_ptr"
-  "irq_cnode_ptr \<notin> tcb_offs_range High_tcb_ptr"
+  "init_irq_node_ptr \<notin> tcb_offs_range High_tcb_ptr"
   "ntfn_ptr \<notin> tcb_offs_range High_tcb_ptr"
   "High_tcb_ptr \<notin> tcb_offs_range idle_tcb_ptr"
   "Low_tcb_ptr \<notin> tcb_offs_range idle_tcb_ptr"
   "High_pool_ptr \<notin> tcb_offs_range idle_tcb_ptr"
   "Low_pool_ptr \<notin> tcb_offs_range idle_tcb_ptr"
-  "irq_cnode_ptr \<notin> tcb_offs_range idle_tcb_ptr"
+  "init_irq_node_ptr \<notin> tcb_offs_range idle_tcb_ptr"
   "ntfn_ptr \<notin> tcb_offs_range idle_tcb_ptr"
   "idle_tcb_ptr \<notin> page_offs_range shared_page_ptr_virt"
   "High_tcb_ptr \<notin> page_offs_range shared_page_ptr_virt"
   "Low_tcb_ptr \<notin> page_offs_range shared_page_ptr_virt"
   "High_pool_ptr \<notin> page_offs_range shared_page_ptr_virt"
   "Low_pool_ptr \<notin> page_offs_range shared_page_ptr_virt"
-  "irq_cnode_ptr \<notin> page_offs_range shared_page_ptr_virt"
+  "init_irq_node_ptr \<notin> page_offs_range shared_page_ptr_virt"
   "ntfn_ptr \<notin> page_offs_range shared_page_ptr_virt"
   by (auto simp: tcb_offs_range_def pt_offs_range_def page_offs_range_def
                  cnode_offs_range_def kh0H_obj_def s0_ptr_defs)
@@ -977,9 +976,11 @@ lemma kh0H_dom_sets_distinct:
   "tcb_offs_range Low_tcb_ptr \<inter> tcb_offs_range idle_tcb_ptr = {}"
   "tcb_offs_range Low_tcb_ptr \<inter> page_offs_range shared_page_ptr_virt = {}"
   "page_offs_range shared_page_ptr_virt \<inter> tcb_offs_range idle_tcb_ptr = {}"
-  by (rule disjointI, clarsimp simp: tcb_offs_range_def pt_offs_range_def page_offs_range_def
-                                     irq_node_offs_range_def cnode_offs_range_def s0_ptr_defs
-                    , drule (1) order_trans le_less_trans, fastforce)+
+  by (rule disjointI,
+      clarsimp simp: tcb_offs_range_def pt_offs_range_def page_offs_range_def
+                     irq_node_offs_range_def cnode_offs_range_def s0_ptr_defs
+                     irq_node_size_def irq_len_val cte_level_bits_def,
+      drule (1) order_trans le_less_trans, fastforce)+
 
 lemmas offs_in_range =
   pt_offs_in_range page_offs_in_range tcb_offs_in_range cnode_offs_in_range irq_node_offs_in_range
@@ -996,63 +997,63 @@ lemma kh0H_dom_distinct':
   "length x = 10 \<Longrightarrow> Silc_cnode_ptr + of_bl x * 0x20 \<noteq> Low_tcb_ptr"
   "length x = 10 \<Longrightarrow> Silc_cnode_ptr + of_bl x * 0x20 \<noteq> High_pool_ptr"
   "length x = 10 \<Longrightarrow> Silc_cnode_ptr + of_bl x * 0x20 \<noteq> Low_pool_ptr"
-  "length x = 10 \<Longrightarrow> Silc_cnode_ptr + of_bl x * 0x20 \<noteq> irq_cnode_ptr"
+  "length x = 10 \<Longrightarrow> Silc_cnode_ptr + of_bl x * 0x20 \<noteq> init_irq_node_ptr"
   "length x = 10 \<Longrightarrow> Silc_cnode_ptr + of_bl x * 0x20 \<noteq> ntfn_ptr"
   "length x = 10 \<Longrightarrow> Low_cnode_ptr + of_bl x * 0x20 \<noteq> idle_tcb_ptr"
   "length x = 10 \<Longrightarrow> Low_cnode_ptr + of_bl x * 0x20 \<noteq> High_tcb_ptr"
   "length x = 10 \<Longrightarrow> Low_cnode_ptr + of_bl x * 0x20 \<noteq> High_pool_ptr"
   "length x = 10 \<Longrightarrow> Low_cnode_ptr + of_bl x * 0x20 \<noteq> Low_pool_ptr"
   "length x = 10 \<Longrightarrow> Low_cnode_ptr + of_bl x * 0x20 \<noteq> Low_tcb_ptr"
-  "length x = 10 \<Longrightarrow> Low_cnode_ptr + of_bl x * 0x20 \<noteq> irq_cnode_ptr"
+  "length x = 10 \<Longrightarrow> Low_cnode_ptr + of_bl x * 0x20 \<noteq> init_irq_node_ptr"
   "length x = 10 \<Longrightarrow> Low_cnode_ptr + of_bl x * 0x20 \<noteq> ntfn_ptr"
   "length x = 10 \<Longrightarrow> High_cnode_ptr + of_bl x * 0x20 \<noteq> idle_tcb_ptr"
   "length x = 10 \<Longrightarrow> High_cnode_ptr + of_bl x * 0x20 \<noteq> High_tcb_ptr"
   "length x = 10 \<Longrightarrow> High_cnode_ptr + of_bl x * 0x20 \<noteq> Low_tcb_ptr"
   "length x = 10 \<Longrightarrow> High_cnode_ptr + of_bl x * 0x20 \<noteq> High_pool_ptr"
   "length x = 10 \<Longrightarrow> High_cnode_ptr + of_bl x * 0x20 \<noteq> Low_pool_ptr"
-  "length x = 10 \<Longrightarrow> High_cnode_ptr + of_bl x * 0x20 \<noteq> irq_cnode_ptr"
+  "length x = 10 \<Longrightarrow> High_cnode_ptr + of_bl x * 0x20 \<noteq> init_irq_node_ptr"
   "length x = 10 \<Longrightarrow> High_cnode_ptr + of_bl x * 0x20 \<noteq> ntfn_ptr"
   "Low_pd_ptr + (ucast y << 3) \<noteq> idle_tcb_ptr"
   "Low_pd_ptr + (ucast y << 3) \<noteq> High_tcb_ptr"
   "Low_pd_ptr + (ucast y << 3) \<noteq> Low_tcb_ptr"
   "Low_pd_ptr + (ucast y << 3) \<noteq> High_pool_ptr"
   "Low_pd_ptr + (ucast y << 3) \<noteq> Low_pool_ptr"
-  "Low_pd_ptr + (ucast y << 3) \<noteq> irq_cnode_ptr"
+  "Low_pd_ptr + (ucast y << 3) \<noteq> init_irq_node_ptr"
   "Low_pd_ptr + (ucast y << 3) \<noteq> ntfn_ptr"
   "High_pd_ptr + (ucast y << 3) \<noteq> idle_tcb_ptr"
   "High_pd_ptr + (ucast y << 3) \<noteq> High_tcb_ptr"
   "High_pd_ptr + (ucast y << 3) \<noteq> Low_tcb_ptr"
   "High_pd_ptr + (ucast y << 3) \<noteq> High_pool_ptr"
   "High_pd_ptr + (ucast y << 3) \<noteq> Low_pool_ptr"
-  "High_pd_ptr + (ucast y << 3) \<noteq> irq_cnode_ptr"
+  "High_pd_ptr + (ucast y << 3) \<noteq> init_irq_node_ptr"
   "High_pd_ptr + (ucast y << 3) \<noteq> ntfn_ptr"
   "Low_pt_ptr + (ucast y << 3) \<noteq> idle_tcb_ptr"
   "Low_pt_ptr + (ucast y << 3) \<noteq> High_tcb_ptr"
   "Low_pt_ptr + (ucast y << 3) \<noteq> Low_tcb_ptr"
   "Low_pt_ptr + (ucast y << 3) \<noteq> High_pool_ptr"
   "Low_pt_ptr + (ucast y << 3) \<noteq> Low_pool_ptr"
-  "Low_pt_ptr + (ucast y << 3) \<noteq> irq_cnode_ptr"
+  "Low_pt_ptr + (ucast y << 3) \<noteq> init_irq_node_ptr"
   "Low_pt_ptr + (ucast y << 3) \<noteq> ntfn_ptr"
   "High_pt_ptr + (ucast y << 3) \<noteq> idle_tcb_ptr"
   "High_pt_ptr + (ucast y << 3) \<noteq> High_tcb_ptr"
   "High_pt_ptr + (ucast y << 3) \<noteq> Low_tcb_ptr"
   "High_pt_ptr + (ucast y << 3) \<noteq> High_pool_ptr"
   "High_pt_ptr + (ucast y << 3) \<noteq> Low_pool_ptr"
-  "High_pt_ptr + (ucast y << 3) \<noteq> irq_cnode_ptr"
+  "High_pt_ptr + (ucast y << 3) \<noteq> init_irq_node_ptr"
   "High_pt_ptr + (ucast y << 3) \<noteq> ntfn_ptr"
   "riscv_global_pt_ptr + (ucast y << 3) \<noteq> idle_tcb_ptr"
   "riscv_global_pt_ptr + (ucast y << 3) \<noteq> High_tcb_ptr"
   "riscv_global_pt_ptr + (ucast y << 3) \<noteq> Low_tcb_ptr"
   "riscv_global_pt_ptr + (ucast y << 3) \<noteq> High_pool_ptr"
   "riscv_global_pt_ptr + (ucast y << 3) \<noteq> Low_pool_ptr"
-  "riscv_global_pt_ptr + (ucast y << 3) \<noteq> irq_cnode_ptr"
+  "riscv_global_pt_ptr + (ucast y << 3) \<noteq> init_irq_node_ptr"
   "riscv_global_pt_ptr + (ucast y << 3) \<noteq> ntfn_ptr"
   "shared_page_ptr_virt + (ucast y << 12) \<noteq> idle_tcb_ptr"
   "shared_page_ptr_virt + (ucast y << 12) \<noteq> High_tcb_ptr"
   "shared_page_ptr_virt + (ucast y << 12) \<noteq> Low_tcb_ptr"
   "shared_page_ptr_virt + (ucast y << 12) \<noteq> High_pool_ptr"
   "shared_page_ptr_virt + (ucast y << 12) \<noteq> Low_pool_ptr"
-  "shared_page_ptr_virt + (ucast y << 12) \<noteq> irq_cnode_ptr"
+  "shared_page_ptr_virt + (ucast y << 12) \<noteq> init_irq_node_ptr"
   "shared_page_ptr_virt + (ucast y << 12) \<noteq> ntfn_ptr"
   apply (drule offs_in_range, fastforce simp: kh0H_dom_distinct)+
   apply (cut_tac x=y in offs_in_range(1), fastforce simp: kh0H_dom_distinct)+
@@ -1078,9 +1079,9 @@ lemma shared_pageH_KOUserData[simp]:
 lemma kh0H_simps[simp]:
   fixes y :: pt_index
   shows
-  "kh0H (init_irq_node_ptr + (ucast (irq :: irq) << 5)) = Some (KOCTE (CTE NullCap Null_mdb))"
+  "kh0H (init_irq_node_ptr + (ucast (irq :: irq) << cte_level_bits)) = Some (KOCTE irq_cte)"
   "kh0H ntfn_ptr      = Some (KONotification ntfnH)"
-  "kh0H irq_cnode_ptr = Some (KOCTE irq_cte)"
+  "kh0H init_irq_node_ptr = Some (KOCTE irq_cte)"
   "kh0H Low_pool_ptr  = Some (KOArch Low_poolH)"
   "kh0H High_pool_ptr = Some (KOArch High_poolH)"
   "kh0H Low_tcb_ptr   = Some (KOTCB Low_tcbH)"
@@ -1096,9 +1097,12 @@ lemma kh0H_simps[simp]:
   "kh0H (riscv_global_pt_ptr + (ucast y << 3)) = global_ptH riscv_global_pt_ptr (riscv_global_pt_ptr + (ucast y << 3))"
   "kh0H (shared_page_ptr_virt + (ucast y << 12)) = Some KOUserData"
   supply option.case_cong[cong]
-  apply (fastforce simp: kh0H_def option_update_range_def)
+                  apply (fastforce simp: kh0H_def option_update_range_def)
+                 apply (clarsimp simp: kh0H_def kh0H_dom_distinct option_update_range_def not_in_range_None)
+                apply (clarsimp simp: kh0H_def kh0H_dom_distinct option_update_range_def not_in_range_None)
+                apply (rule_tac x=0 in exI, simp)
   by ((clarsimp simp: kh0H_def kh0H_dom_distinct kh0H_dom_distinct'
-                       option_update_range_def not_in_range_None offs_in_range
+                      option_update_range_def not_in_range_None offs_in_range
        | simp add: offs_in_range kh0H_dom_sets_distinct[THEN orthD1] not_in_range_None
        | simp add: offs_in_range kh0H_dom_sets_distinct[THEN orthD2] not_in_range_None
        | rule conjI | clarsimp split: option.splits)+,
@@ -1109,7 +1113,7 @@ lemma kh0H_simps[simp]:
 
 lemma kh0H_dom:
   "dom kh0H = {idle_tcb_ptr, High_tcb_ptr, Low_tcb_ptr,
-               High_pool_ptr, Low_pool_ptr, irq_cnode_ptr, ntfn_ptr} \<union>
+               High_pool_ptr, Low_pool_ptr, ntfn_ptr} \<union>
               irq_node_offs_range \<union>
               page_offs_range shared_page_ptr_virt \<union>
               cnode_offs_range Silc_cnode_ptr \<union>
@@ -1122,17 +1126,20 @@ lemma kh0H_dom:
               pt_offs_range Low_pt_ptr"
   apply (rule equalityI)
    apply (simp add: kh0H_def dom_def)
-   apply (clarsimp simp: offs_in_range option_update_range_def not_in_range_None split: if_split_asm)
+   apply (clarsimp simp: offs_in_range option_update_range_def not_in_range_None
+                   simp flip: cte_level_bits_def
+                   split: if_split_asm)
   apply (clarsimp simp: dom_def)
   apply (rule conjI)
    apply (force simp: kh0H_def kh0H_dom_distinct option_update_range_def not_in_range_None
+                simp flip: cte_level_bits_def
                 dest: irq_node_offs_range_correct split: option.splits)
   by (rule conjI
       | clarsimp simp: kh0H_def kh0H_dom_distinct option_update_range_def not_in_range_None
-                split: option.splits
-        , frule offs_range_correct
-        , clarsimp simp: kh0H_all_obj_def cnode_offs_range_def page_offs_range_def pt_offs_range_def
-                  split: if_split_asm)+
+                 split: option.splits,
+        frule offs_range_correct,
+        clarsimp simp: kh0H_all_obj_def cnode_offs_range_def page_offs_range_def pt_offs_range_def
+                 split: if_split_asm)+
 
 lemmas kh0H_SomeD' = set_mp[OF equalityD1[OF kh0H_dom[simplified dom_def]], OF CollectI, simplified, OF exI]
 
@@ -1144,7 +1151,7 @@ lemma kh0H_SomeD:
        x = idle_tcb_ptr \<and> y = KOTCB idle_tcbH \<or>
        x \<in> pt_offs_range riscv_global_pt_ptr \<and> global_ptH riscv_global_pt_ptr x \<noteq> None
                                              \<and> y = the (global_ptH riscv_global_pt_ptr x) \<or>
-       x \<in> irq_node_offs_range \<and> y = KOCTE (CTE NullCap Null_mdb) \<or>
+       x \<in> irq_node_offs_range \<and> y = KOCTE irq_cte \<or>
        x \<in> pt_offs_range Low_pt_ptr \<and> Low_ptH Low_pt_ptr x \<noteq> None \<and> y = the (Low_ptH Low_pt_ptr x) \<or>
        x \<in> pt_offs_range High_pt_ptr \<and> High_ptH High_pt_ptr x \<noteq> None \<and> y = the (High_ptH High_pt_ptr x) \<or>
        x \<in> pt_offs_range Low_pd_ptr \<and> Low_pdH Low_pd_ptr x \<noteq> None \<and> y = the (Low_pdH Low_pd_ptr x) \<or>
@@ -1154,7 +1161,6 @@ lemma kh0H_SomeD:
        x \<in> cnode_offs_range Low_cnode_ptr \<and> Low_cte Low_cnode_ptr x \<noteq> None \<and> y = the (Low_cte Low_cnode_ptr x) \<or>
        x \<in> cnode_offs_range High_cnode_ptr \<and> High_cte High_cnode_ptr x \<noteq> None \<and> y = the (High_cte High_cnode_ptr x) \<or>
        x \<in> cnode_offs_range Silc_cnode_ptr \<and> Silc_cte Silc_cnode_ptr x \<noteq> None \<and> y = the (Silc_cte Silc_cnode_ptr x) \<or>
-       x = irq_cnode_ptr \<and> y = KOCTE irq_cte \<or>
        x \<in> page_offs_range shared_page_ptr_virt \<and> y = KOUserData"
   apply (frule kh0H_SomeD')
   apply (elim disjE)
@@ -1172,12 +1178,12 @@ definition s0H_internal :: "kernel_state" where
   "s0H_internal \<equiv> \<lparr>
      ksPSpace = kh0H,
      gsUserPages = [shared_page_ptr_virt \<mapsto> RISCVLargePage],
-     gsCNodes = (\<lambda>x. if \<exists>irq :: irq. init_irq_node_ptr + (ucast irq << 5) = x
+     gsCNodes = (\<lambda>x. if \<exists>irq :: irq. init_irq_node_ptr + (ucast irq << cte_level_bits) = x
                      then Some 0 else None)
                 (Low_cnode_ptr  \<mapsto> 10,
                  High_cnode_ptr \<mapsto> 10,
                  Silc_cnode_ptr \<mapsto> 10,
-                 irq_cnode_ptr  \<mapsto> 0),
+                 init_irq_node_ptr  \<mapsto> 0),
      gsUntypedZeroRanges = ran (map_comp untypedZeroRange (option_map cteCap o map_to_ctes kh0H)),
      gsMaxObjectSize = card (UNIV :: obj_ref set),
      ksDomScheduleIdx = 0,
@@ -1198,16 +1204,16 @@ definition s0H_internal :: "kernel_state" where
 
 
 definition Low_cte_cte :: "obj_ref \<Rightarrow> obj_ref \<Rightarrow> cte option" where
-  "Low_cte_cte \<equiv> \<lambda>base offs. if is_aligned offs 5 \<and> base \<le> offs \<and> offs \<le> base + 2 ^ 15 - 1
-                              then Low_cte' (ucast (offs - base >> 5)) else None"
+  "Low_cte_cte \<equiv> \<lambda>base offs. if is_aligned offs cte_level_bits \<and> base \<le> offs \<and> offs \<le> base + 2 ^ 15 - 1
+                              then Low_cte' (ucast (offs - base >> cte_level_bits)) else None"
 
 definition High_cte_cte :: "obj_ref \<Rightarrow> obj_ref \<Rightarrow> cte option" where
-  "High_cte_cte \<equiv> \<lambda>base offs. if is_aligned offs 5 \<and> base \<le> offs \<and> offs \<le> base + 2 ^ 15 - 1
-                               then High_cte' (ucast (offs - base >> 5)) else None"
+  "High_cte_cte \<equiv> \<lambda>base offs. if is_aligned offs cte_level_bits \<and> base \<le> offs \<and> offs \<le> base + 2 ^ 15 - 1
+                               then High_cte' (ucast (offs - base >> cte_level_bits)) else None"
 
 definition Silc_cte_cte :: "obj_ref \<Rightarrow> obj_ref \<Rightarrow> cte option" where
-  "Silc_cte_cte \<equiv> \<lambda>base offs. if is_aligned offs 5 \<and> base \<le> offs \<and> offs \<le> base + 2 ^ 15 - 1
-                               then Silc_cte' (ucast (offs - base >> 5)) else None"
+  "Silc_cte_cte \<equiv> \<lambda>base offs. if is_aligned offs cte_level_bits \<and> base \<le> offs \<and> offs \<le> base + 2 ^ 15 - 1
+                               then Silc_cte' (ucast (offs - base >> cte_level_bits)) else None"
 
 definition Low_tcb_cte :: "obj_ref \<Rightarrow> cte option" where
   "Low_tcb_cte \<equiv> [Low_tcb_ptr \<mapsto> tcbCTable Low_tcbH,
@@ -1252,13 +1258,138 @@ lemma set_mem_neq:
   "\<lbrakk> y \<notin> S; x \<in> S \<rbrakk> \<Longrightarrow> x \<noteq> y"
   by fastforce
 
-lemma neg_mask_decompose:
+lemma neg_mask_decompose: (* FIXME: move to WordLib *)
   "x && ~~ mask n = ptr \<Longrightarrow> x = ptr + (x && mask n)"
   by (clarsimp simp: AND_NOT_mask_plus_AND_mask_eq)
 
 lemma opt_None_not_dom:
   "m a = None \<Longrightarrow> a \<notin> dom m"
   by (simp add: dom_def)
+
+
+lemma kh_s0H[simp]:
+  "ksPSpace s0H_internal = kh0H"
+  by (simp add: s0H_internal_def)
+
+lemma s0H_pspace_aligned'[intro!]:
+  "pspace_aligned' s0H_internal"
+  supply [simp] = cte_level_bits_def pteBits_def objBits_defs
+  apply (clarsimp simp: pspace_aligned'_def)
+  apply (drule kh0H_SomeD)
+  by (elim disjE; clarsimp simp: s0_ptr_defs kh0H_all_obj_def objBitsKO_def archObjSize_def
+                                 cnode_offs_range_def page_offs_range_def pt_offs_range_def
+                                 irq_node_offs_range_def is_aligned_mask mask_def bit_simps
+                           split: if_splits)
+
+interpretation sorted_addrs objBitsKO .
+
+lemma pspace_aligned'_obj_aligned:
+  "\<lbrakk> pspace_aligned' s; set addrs = dom (ksPSpace s) \<rbrakk> \<Longrightarrow> obj_aligned (ksPSpace s) addrs"
+  unfolding obj_aligned_def pspace_aligned'_def align_of_def
+  by force
+
+lemma init_irq_node_ptr_less_size_eq_le_mask:
+  "(x < init_irq_node_ptr + irq_node_size) =
+   (x \<le> init_irq_node_ptr + mask (irq_len + cte_level_bits))"
+  apply (simp add: init_irq_node_ptr_def irq_node_size_def irq_len_val cte_level_bits_def mask_def
+                   pptr_base_def pptrBase_def canonical_bit_def)
+  apply unat_arith
+  done
+
+lemma aligned_offsets_irq_node_offs_range:
+  "set (aligned_offsets init_irq_node_ptr (irq_len + cte_level_bits) cte_level_bits) =
+   irq_node_offs_range"
+  by (simp add: set_aligned_offsets irq_node_offs_range_def init_irq_node_ptr_less_size_eq_le_mask)
+
+lemma aligned_offsets_page_offs_range:
+  "is_aligned p pageBits \<Longrightarrow> set (aligned_offsets p 21 pageBits) = page_offs_range p"
+  by (simp add: set_aligned_offsets page_offs_range_def mask_def add.commute pageBits_def)
+
+lemma aligned_offsets_cnode_offs_range:
+  "is_aligned p cte_level_bits \<Longrightarrow> set (aligned_offsets p 15 cte_level_bits) = cnode_offs_range p"
+  by (simp add: set_aligned_offsets cnode_offs_range_def mask_def add.commute)
+
+lemma aligned_offsets_pt_offs_range:
+  "is_aligned p pte_bits \<Longrightarrow> set (aligned_offsets p 12 pte_bits) = pt_offs_range p"
+  by (simp add: set_aligned_offsets pt_offs_range_def mask_def add.commute bit_simps)
+
+definition kh0H_addrs :: "obj_ref list" where
+  "kh0H_addrs = [ntfn_ptr, Low_tcb_ptr, High_tcb_ptr, idle_tcb_ptr] @
+                aligned_offsets riscv_global_pt_ptr 12 pte_bits @
+                aligned_offsets Low_pt_ptr 12 pte_bits @
+                aligned_offsets High_pt_ptr 12 pte_bits @
+                aligned_offsets Low_pd_ptr 12 pte_bits @
+                aligned_offsets High_pd_ptr 12 pte_bits @
+                [Low_pool_ptr, High_pool_ptr] @
+                aligned_offsets Low_cnode_ptr 15 cte_level_bits @
+                aligned_offsets High_cnode_ptr 15 cte_level_bits @
+                aligned_offsets Silc_cnode_ptr 15 cte_level_bits @
+                aligned_offsets init_irq_node_ptr (irq_len + cte_level_bits) cte_level_bits @
+                aligned_offsets shared_page_ptr_virt 21 pageBits"
+
+lemma s0_pt_ptrs_aligned_pte_bits[simp]:
+  "is_aligned riscv_global_pt_ptr pte_bits"
+  "is_aligned Low_pt_ptr pte_bits"
+  "is_aligned High_pt_ptr pte_bits"
+  "is_aligned Low_pd_ptr pte_bits"
+  "is_aligned High_pd_ptr pte_bits"
+  "is_aligned Low_cnode_ptr cte_level_bits"
+  "is_aligned High_cnode_ptr cte_level_bits"
+  "is_aligned Silc_cnode_ptr cte_level_bits"
+  "is_aligned shared_page_ptr_virt pageBits"
+  by (rule is_aligned_weaken, rule s0_ptrs_aligned, simp add: bit_simps cte_level_bits_def)+
+
+lemma offsets_align_s0_ptrs[simp, intro!]:
+  "offsets_align kh0H (set (aligned_offsets riscv_global_pt_ptr 12 pte_bits)) pte_bits"
+  "offsets_align kh0H (set (aligned_offsets Low_pt_ptr 12 pte_bits)) pte_bits"
+  "offsets_align kh0H (set (aligned_offsets High_pt_ptr 12 pte_bits)) pte_bits"
+  "offsets_align kh0H (set (aligned_offsets Low_pd_ptr 12 pte_bits)) pte_bits"
+  "offsets_align kh0H (set (aligned_offsets High_pd_ptr 12 pte_bits)) pte_bits"
+  "offsets_align kh0H (set (aligned_offsets shared_page_ptr_virt 21 pageBits)) pageBits"
+  "offsets_align kh0H (set (aligned_offsets Low_cnode_ptr 15 cte_level_bits)) cte_level_bits"
+  "offsets_align kh0H (set (aligned_offsets High_cnode_ptr 15 cte_level_bits)) cte_level_bits"
+  "offsets_align kh0H (set (aligned_offsets Silc_cnode_ptr 15 cte_level_bits)) cte_level_bits"
+  "offsets_align kh0H
+                 (set (aligned_offsets init_irq_node_ptr (irq_len + cte_level_bits) cte_level_bits))
+                 cte_level_bits"
+  using aligned_offsets_pt_offs_range aligned_offsets_page_offs_range
+        aligned_offsets_cnode_offs_range aligned_offsets_irq_node_offs_range
+        cteSizeBits_cte_level_bits
+  by (clarsimp simp: offsets_align_def s0_ptrs_aligned align_of_def,
+      prop_tac "p \<in> dom kh0H", simp add: kh0H_dom,
+      clarsimp simp: kh0H_obj_def objBits_simps dest!: offs_range_correct split: if_splits)+
+
+lemma cte_level_bits_le_cnode_size[simp]:
+  "cte_level_bits \<le> 15"
+  by (simp add: cte_level_bits_def)
+
+lemma pte_bits_le_pt_size[simp]:
+  "pte_bits \<le> 12"
+  by (simp add: pte_bits_def bit_simps)
+
+lemma obj_spaced_kh0H_addrs:
+  "obj_spaced kh0H kh0H_addrs"
+  supply [simp] = irq_cte_len_leq_word[simplified] s0_ptrs_aligned aligned_offsets_neq_Nil
+  apply (simp add: kh0H_addrs_def obj_spaced_cons_aligned_offsets obj_spaced_append)
+  apply (simp add: hd_aligned_offsets hd_aligned_offsets_append)
+  apply (simp add: aligned_offsets_obj_spaced last_aligned_offests_plus_mask)
+  apply (simp add: align_of_def objBitsKO_def objBits_defs kh0H_obj_def archObjSize_def bit_simps)
+  by (simp add: s0_ptr_defs mask_def irq_len_val cte_level_bits_def) (* arithmetic only *)
+
+lemma dom_eq_kh0H_addrs:
+  "dom kh0H = set kh0H_addrs"
+  by (auto simp: kh0H_dom kh0H_addrs_def aligned_offsets_irq_node_offs_range
+                 aligned_offsets_cnode_offs_range aligned_offsets_pt_offs_range
+                 aligned_offsets_page_offs_range)
+
+lemma s0H_pspace_distinct':
+  "pspace_distinct' s0H_internal"
+  apply (clarsimp simp: pspace_distinct'_def ps_clear_def)
+  apply (rule obj_spaced_distinct[where addrs=kh0H_addrs];
+         clarsimp simp: dom_eq_kh0H_addrs obj_spaced_kh0H_addrs
+                        pspace_aligned'_obj_aligned[where s=s0H_internal, simplified]
+                        s0H_pspace_aligned')
+  done
 
 lemma tcb_offs_range_mask_eq:
   "\<lbrakk> x \<in> tcb_offs_range ptr; is_aligned ptr 10 \<rbrakk> \<Longrightarrow> x && ~~ mask 10 = ptr"
@@ -1330,18 +1461,54 @@ lemma kh0H_dom_tcb:
    \<Longrightarrow> x = Low_tcb_ptr \<or> x = High_tcb_ptr \<or> x = idle_tcb_ptr"
   apply (frule domI[where m="kh0H"])
   apply (simp add: kh0H_dom)
-  apply (elim disjE)
-  by (auto dest: offs_range_correct simp: kh0H_all_obj_def s0_ptrs_aligned split: if_split_asm)
+  apply (auto dest: offs_range_correct simp: kh0H_all_obj_def s0_ptrs_aligned split: if_split_asm)
+  done
+
+lemma kh0H_ko_aligned:
+  "kh0H p = Some ko \<Longrightarrow> is_aligned p (objBitsKO ko)"
+  using s0H_pspace_aligned'
+  by (force simp: pspace_aligned'_def)
+
+lemma kh0H_ko_distinct:
+  "kh0H p = Some ko \<Longrightarrow> (mask_range p (objBitsKO ko) - {p}) \<inter> dom kh0H = {}"
+  using s0H_pspace_distinct'
+  by (fastforce simp: pspace_distinct'_def ps_clear_def)
+
+lemma kh0H_cte_aligned:
+  "kh0H p = Some (KOCTE cte) \<Longrightarrow> is_aligned p cte_level_bits"
+  by (clarsimp dest!: kh0H_ko_aligned simp: objBitsKO_def cteSizeBits_cte_level_bits)
+
+lemma kh0H_cte_distinct:
+  "kh0H p = Some (KOCTE cte) \<Longrightarrow> (mask_range p cte_level_bits - {p}) \<inter> dom kh0H = {}"
+  by (clarsimp dest!: kh0H_ko_distinct simp: objBitsKO_def cteSizeBits_cte_level_bits)
+
+lemma aligned_plus_1_eq_mask_range:
+  "\<lbrakk> is_aligned p n; 0 < n \<rbrakk> \<Longrightarrow> {p + 1..p + mask n} = mask_range p n - {p}"
+  apply (rule equalityI; clarsimp)
+   apply (metis aligned_less_plus_1 word_add_increasing word_le_less_eq word_not_le)
+  apply (metis plus_one_helper word_le_less_eq word_not_le)
+  done
+
+lemma kh0_cte_map_to_ctes:
+  "kh0H p = Some (KOCTE cte) \<Longrightarrow> map_to_ctes kh0H p = Some cte"
+  apply (frule kh0H_cte_aligned)
+  apply (frule kh0H_cte_distinct)
+  apply (clarsimp simp: map_to_ctes_def Let_def objBitsKO_def cteSizeBits_cte_level_bits
+                        add_mask_fold aligned_plus_1_eq_mask_range)
+  done
+
+lemma subset_not_disjointD:
+  "\<lbrakk> A \<inter> C = {}; B \<inter> C \<noteq> {}; B \<subseteq> A \<rbrakk> \<Longrightarrow> False"
+  by blast
 
 lemma map_to_ctes_kh0H:
   "map_to_ctes kh0H =
      (option_update_range
-        (\<lambda>x. if \<exists>irq :: irq. init_irq_node_ptr + (ucast irq << 5) = x
-             then Some (CTE NullCap Null_mdb) else None) \<circ>
+        (\<lambda>x. if \<exists>irq :: irq. init_irq_node_ptr + (ucast irq << cte_level_bits) = x
+             then Some irq_cte else None) \<circ>
       option_update_range (Low_cte_cte Low_cnode_ptr) \<circ>
       option_update_range (High_cte_cte High_cnode_ptr) \<circ>
       option_update_range (Silc_cte_cte Silc_cnode_ptr) \<circ>
-      option_update_range [irq_cnode_ptr \<mapsto> CTE NullCap Null_mdb] \<circ>
       option_update_range Low_tcb_cte \<circ>
       option_update_range High_tcb_cte \<circ>
       option_update_range idle_tcb_cte
@@ -1358,7 +1525,6 @@ lemma map_to_ctes_kh0H:
     apply (elim disjE)
       apply (clarsimp simp: option_update_range_def)
       apply (frule mask_in_tcb_offs_range)
-      apply (clarsimp simp: kh0H_dom_distinct[THEN set_mem_neq])
       apply (simp add: kh0H_dom_sets_distinct[THEN orthD2] not_in_range_cte_None
              | simp add: kh0H_dom_sets_distinct[THEN orthD1] not_in_range_cte_None)+
       apply (rule conjI, clarsimp)
@@ -1369,7 +1535,6 @@ lemma map_to_ctes_kh0H:
                            split: if_split_asm dest: neg_mask_decompose)
      apply (clarsimp simp: option_update_range_def)
      apply (frule mask_in_tcb_offs_range)
-     apply (clarsimp simp: kh0H_dom_distinct[THEN set_mem_neq])
      apply (simp add: kh0H_dom_sets_distinct[THEN orthD2] not_in_range_cte_None
             | simp add: kh0H_dom_sets_distinct[THEN orthD1] not_in_range_cte_None)+
      apply (rule conjI, clarsimp)
@@ -1381,7 +1546,6 @@ lemma map_to_ctes_kh0H:
                           split: if_split_asm dest: neg_mask_decompose)
     apply (clarsimp simp: option_update_range_def)
     apply (frule mask_in_tcb_offs_range)
-    apply (clarsimp simp: kh0H_dom_distinct[THEN set_mem_neq])
     apply (simp add: kh0H_dom_sets_distinct[THEN orthD2] not_in_range_cte_None
            | simp add: kh0H_dom_sets_distinct[THEN orthD1] not_in_range_cte_None)+
     apply (rule conjI, clarsimp)
@@ -1440,42 +1604,40 @@ lemma map_to_ctes_kh0H:
                        clarsimp simp: option_update_range_def kh0H_dom_distinct[THEN set_mem_neq] not_in_range_cte_None,
                        ((clarsimp simp: kh0H_dom_sets_distinct[THEN orthD1] not_in_range_cte_None irq_node_offs_in_range |
                          clarsimp simp: kh0H_dom_sets_distinct[THEN orthD2] not_in_range_cte_None)+)[1])+)[5]
-          prefer 8
+          prefer 7
           apply ((clarsimp simp: map_to_ctes_def Let_def kh0H_obj_def split del: if_split,
                   subst if_split_eq1, rule conjI,
                   clarsimp, drule kh0H_dom_tcb, fastforce simp: s0_ptr_defs mask_def objBitsKO_def,
                   fastforce simp: option_update_range_def kh0H_dom_distinct not_in_range_cte_None)+)[3]
-       apply ((clarsimp simp: map_to_ctes_def Let_def kh0H_obj_def objBitsKO_def
-                       split: if_split_asm split del: if_split,
-               subst if_split_eq1, rule conjI, rule impI,
-               clarsimp simp: option_update_range_def kh0H_dom_distinct not_in_range_cte_None,
-               (clarsimp simp: option_update_range_def kh0H_dom_distinct[THEN set_mem_neq]
-                               kh0H_dom_sets_distinct[THEN orthD1] not_in_range_cte_None
-                | simp add: kh0H_dom_sets_distinct[THEN orthD2] not_in_range_cte_None)+,
-               rule conjI, clarsimp, drule offs_range_correct,
-               fastforce simp: Low_cte_cte_def High_cte_cte_def Silc_cte_cte_def,
-               rule impI, rule FalseE, drule offs_range_correct,
-               clarsimp simp: Low_cte_def High_cte_def Silc_cte_def cnode_offs_min cnode_offs_max,
-               cut_tac x="of_bl y" and z="0x20::obj_ref" and y="2 ^ 15 - 1" in div_to_mult_word_lt,
-               frule_tac 'a=64 in of_bl_length_le, simp, simp, drule int_not_emptyD,
-               clarsimp simp: kh0H_dom s0_ptr_defs cnode_offs_range_def page_offs_range_def
-                              pt_offs_range_def irq_node_offs_range_def,
-               (elim disjE, (clarsimp simp: s0_ptr_defs,
-                             drule_tac b="x + y * 0x20" and n=5 for x y in aligned_le_sharp,
-                             fastforce simp: is_aligned_def, clarsimp simp: add.commute,
-                             subst (asm) mask_out_add_aligned[symmetric],
-                             simp add: is_aligned_mult_triv2[where n=5, simplified],
-                             simp add: mask_def, drule word_leq_le_minus_one,
-                             subst add.commute, rule neq_0_no_wrap,
-                             erule word_plus_mono_right2[rotated],
-                             fastforce, fastforce, fastforce simp: add.commute | unat_arith)+)[1])+)[3]
-    apply (clarsimp simp: map_to_ctes_def Let_def kh0H_obj_def split del: if_split,
-           subst if_split_eq1, rule conjI, rule impI,
-           clarsimp simp: option_update_range_def kh0H_dom_distinct not_in_range_cte_None, rule impI,
-           clarsimp simp: kh0H_dom objBitsKO_def s0_ptr_defs is_aligned_def page_offs_range_def
-                          cnode_offs_range_def pt_offs_range_def irq_node_offs_range_def,
-           rule FalseE, drule int_not_emptyD, clarsimp,
-           (elim disjE, (clarsimp | drule(1) order_trans le_less_trans, fastforce)+)[1])
+      (* Low_cnode *)
+      apply (clarsimp simp: Low_cte_def split: if_split_asm)
+      apply (frule kh0_cte_map_to_ctes)
+      apply (clarsimp simp: option_update_range_def)
+      apply (fastforce simp: Low_cte_cte_def)
+     (* High_cnode *)
+     apply (clarsimp simp: High_cte_def split: if_split_asm)
+     apply (frule kh0_cte_map_to_ctes)
+     apply (clarsimp simp: option_update_range_def)
+     apply (rename_tac p cte)
+     apply (rule conjI; clarsimp)
+     apply (prop_tac "Low_cte_cte Low_cnode_ptr p = None")
+      apply (rule not_in_range_cte_None)
+      apply (erule kh0H_dom_sets_distinct[THEN orthD1])
+     apply (clarsimp simp: High_cte_cte_def split: option.split)
+    (* Silc_cnode *)
+    apply (clarsimp simp: Silc_cte_def split: if_split_asm)
+    apply (frule kh0_cte_map_to_ctes)
+    apply (clarsimp simp: option_update_range_def)
+    apply (rename_tac p cte)
+    apply (rule conjI; clarsimp)
+    apply (prop_tac "Low_cte_cte Low_cnode_ptr p = None")
+     apply (rule not_in_range_cte_None)
+     apply (erule kh0H_dom_sets_distinct[THEN orthD1])
+    apply (prop_tac "High_cte_cte High_cnode_ptr p = None")
+     apply (rule not_in_range_cte_None)
+     apply (erule kh0H_dom_sets_distinct[THEN orthD1])
+    apply (clarsimp simp: Silc_cte_cte_def split: option.split)
+   (* shared_page_ptr_virt *)
    apply (clarsimp simp: map_to_ctes_def Let_def kh0H_obj_def split del: if_split)
    apply (subst if_split_eq1)
    apply (rule conjI, clarsimp)
@@ -1483,53 +1645,26 @@ lemma map_to_ctes_kh0H:
    apply (clarsimp simp: option_update_range_def kh0H_dom_distinct not_in_range_cte_None)
    apply (rule conjI; clarsimp)
    apply (rule conjI; clarsimp)
-   apply (subst is_aligned_neg_mask_eq, clarsimp simp: objBitsKO_def page_offs_range_def is_aligned_weaken)+
-   apply (clarsimp split: option.splits)
-   apply (intro conjI impI; drule kh0H_dom_sets_distinct[THEN orthD2]
-                                  kh0H_dom_sets_distinct[THEN orthD1],
-                            drule not_in_range_cte_None, solves clarsimp)
-  apply (clarsimp simp: map_to_ctes_def Let_def kh0H_obj_def split del: if_split)
+    apply (clarsimp split: option.split)
+    apply (intro conjI impI; drule kh0H_dom_sets_distinct[THEN orthD2]
+                                   kh0H_dom_sets_distinct[THEN orthD1],
+                             drule not_in_range_cte_None, solves clarsimp)
+   apply (clarsimp simp: page_offs_range_def add_mask_fold)
+   apply (subst (asm) aligned_plus_1_eq_mask_range, simp)
+    apply (simp add: objBitsKO_def)
+   apply (frule kh0H_ko_aligned)
+   apply (frule kh0H_ko_distinct)
+   apply (simp add: objBitsKO_def pageBits_def)
+   apply (drule (1) subset_not_disjointD)
+    apply (rule Diff_mono; clarsimp)
+    apply (rule aligned_mask_step; clarsimp simp: is_aligned_weaken is_aligned_no_overflow_mask)
+   apply (erule FalseE)
+  (* init_irq_cnode *)
+  apply clarsimp
+  apply (frule kh0_cte_map_to_ctes)
+  apply (clarsimp simp: option_update_range_def)
   apply (frule irq_node_offs_range_correct)
-  apply (subst if_split_eq1)
-  apply (rule conjI)
-   apply (rule impI)
-   apply (clarsimp simp: option_update_range_def kh0H_dom_distinct not_in_range_cte_None)
-   apply fastforce
-  apply (rule impI)
-  apply clarsimp
-  apply (erule impE)
-   apply (rule is_aligned_add)
-    apply (simp add: is_aligned_def s0_ptr_defs objBitsKO_def)
-   apply (rule is_aligned_shiftl)
-   apply (clarsimp simp: objBitsKO_def)
-  apply (rule FalseE)
-  apply (clarsimp simp: s0_ptr_defs cnode_offs_range_def page_offs_range_def pt_offs_range_def
-                        irq_node_offs_range_def objBitsKO_def kh0H_dom)
-  apply (cut_tac x=irq and 'a=64 in ucast_less)
-   apply simp
-  apply (drule shiftl_less_t2n'[where n=5])
-   apply simp
-  apply simp
-  apply (drule plus_one_helper[where n="0x7FF", simplified])
-  apply (elim disjE)
-         apply (unat_arith+)[7]
-  apply (drule int_not_emptyD)
-  apply clarsimp
-  apply (elim disjE,
-         ((clarsimp,
-          drule(1) aligned_le_sharp,
-          clarsimp simp: add.commute,
-          subst(asm) mask_out_add_aligned[symmetric],
-           simp add: is_aligned_shiftl,
-          simp add: mask_def,
-          drule word_leq_le_minus_one,
-           subst add.commute,
-           rule neq_0_no_wrap,
-            erule word_plus_mono_right2[rotated],
-            fastforce,
-           fastforce,
-          fastforce simp: add.commute)
-          | unat_arith)+)[1]
+  apply fastforce
   done
 
 lemma option_update_range_map_comp:
@@ -1541,8 +1676,8 @@ lemma tcb_offs_in_rangeI:
   by (simp add: tcb_offs_range_def)
 
 lemma map_to_ctes_kh0H_simps[simp]:
-  "map_to_ctes kh0H (init_irq_node_ptr + (ucast (irq :: irq) << 5)) = Some (CTE NullCap Null_mdb)"
-  "map_to_ctes kh0H irq_cnode_ptr = Some (CTE NullCap Null_mdb)"
+  "map_to_ctes kh0H (init_irq_node_ptr + (ucast (irq :: irq) << cte_level_bits)) =
+     Some irq_cte"
   "length x = 10 \<Longrightarrow> map_to_ctes kh0H (Low_cnode_ptr + of_bl x * 0x20) =
                      Low_cte_cte Low_cnode_ptr (Low_cnode_ptr + of_bl x * 0x20)"
   "length x = 10 \<Longrightarrow> map_to_ctes kh0H (High_cnode_ptr + of_bl x * 0x20) =
@@ -1564,10 +1699,9 @@ lemma map_to_ctes_kh0H_simps[simp]:
   "map_to_ctes kh0H (idle_tcb_ptr + 0x40) = idle_tcb_cte (idle_tcb_ptr + 0x40)"
   "map_to_ctes kh0H (idle_tcb_ptr + 0x60) = idle_tcb_cte (idle_tcb_ptr + 0x60)"
   "map_to_ctes kh0H (idle_tcb_ptr + 0x80) = idle_tcb_cte (idle_tcb_ptr + 0x80)"
-  supply option.case_cong[cong] if_cong[cong]
-     apply (clarsimp simp: map_to_ctes_kh0H option_update_range_def)
-     apply fastforce
-    apply (clarsimp simp: map_to_ctes_kh0H option_update_range_def kh0H_dom_distinct not_in_range_cte_None)
+                    supply option.case_cong[cong] if_cong[cong]
+                    apply (clarsimp simp: map_to_ctes_kh0H option_update_range_def)
+                    apply fastforce
    apply ((clarsimp simp: option_update_range_def not_in_range_cte_None cnode_offs_in_range
                           kh0H_dom_distinct kh0H_dom_distinct' map_to_ctes_kh0H s0_ptrs_aligned,
            ((clarsimp simp: offs_in_range kh0H_dom_sets_distinct[THEN orthD1] not_in_range_cte_None |
@@ -1587,7 +1721,6 @@ lemma map_to_ctes_kh0H_simps[simp]:
   apply ((simp add: offs_in_range kh0H_dom_sets_distinct[THEN orthD1] not_in_range_cte_None
         | simp add: offs_in_range kh0H_dom_sets_distinct[THEN orthD2] not_in_range_cte_None)+)[1]
   apply (intro conjI impI allI)
-     apply (simp add: s0_ptr_defs)
     apply clarsimp
     apply (drule not_disjointI,
              rule irq_node_offs_in_range,
@@ -1595,7 +1728,6 @@ lemma map_to_ctes_kh0H_simps[simp]:
            erule notE,
            rule kh0H_dom_sets_distinct)
    apply (clarsimp simp: kh0H_dom_distinct)
-  apply clarsimp
   apply (drule not_disjointI,
            rule irq_node_offs_in_range,
           assumption,
@@ -1608,7 +1740,6 @@ lemma map_to_ctes_kh0H_simps[simp]:
   apply ((simp add: offs_in_range kh0H_dom_sets_distinct[THEN orthD1] not_in_range_cte_None
         | simp add: offs_in_range kh0H_dom_sets_distinct[THEN orthD2] not_in_range_cte_None)+)[1]
   apply (intro conjI impI allI)
-     apply (simp add: s0_ptr_defs)
     apply clarsimp
     apply (drule not_disjointI,
              rule irq_node_offs_in_range,
@@ -1616,7 +1747,6 @@ lemma map_to_ctes_kh0H_simps[simp]:
            erule notE,
            rule kh0H_dom_sets_distinct)
    apply (clarsimp simp: kh0H_dom_distinct)
-  apply clarsimp
   apply (drule not_disjointI,
            rule irq_node_offs_in_range,
           assumption,
@@ -1629,7 +1759,6 @@ lemma map_to_ctes_kh0H_simps[simp]:
   apply ((simp add: offs_in_range kh0H_dom_sets_distinct[THEN orthD1] not_in_range_cte_None
         | simp add: offs_in_range kh0H_dom_sets_distinct[THEN orthD2] not_in_range_cte_None)+)[1]
   apply (intro conjI impI allI)
-     apply (simp add: s0_ptr_defs)
     apply clarsimp
     apply (drule not_disjointI,
              rule irq_node_offs_in_range,
@@ -1637,7 +1766,6 @@ lemma map_to_ctes_kh0H_simps[simp]:
            erule notE,
            rule kh0H_dom_sets_distinct)
    apply (clarsimp simp: kh0H_dom_distinct)
-  apply clarsimp
   apply (drule not_disjointI,
            rule irq_node_offs_in_range,
           assumption,
@@ -1650,7 +1778,6 @@ lemma map_to_ctes_kh0H_simps[simp]:
   apply ((simp add: offs_in_range kh0H_dom_sets_distinct[THEN orthD1] not_in_range_cte_None
         | simp add: offs_in_range kh0H_dom_sets_distinct[THEN orthD2] not_in_range_cte_None)+)[1]
   apply (intro conjI impI allI)
-     apply (simp add: s0_ptr_defs)
     apply clarsimp
     apply (drule not_disjointI,
              rule irq_node_offs_in_range,
@@ -1658,7 +1785,6 @@ lemma map_to_ctes_kh0H_simps[simp]:
            erule notE,
            rule kh0H_dom_sets_distinct)
    apply (clarsimp simp: kh0H_dom_distinct)
-  apply clarsimp
   apply (drule not_disjointI,
            rule irq_node_offs_in_range,
           assumption,
@@ -1672,7 +1798,6 @@ lemma map_to_ctes_kh0H_simps[simp]:
   apply ((simp add: offs_in_range kh0H_dom_sets_distinct[THEN orthD1] not_in_range_cte_None
         | simp add: offs_in_range kh0H_dom_sets_distinct[THEN orthD2] not_in_range_cte_None)+)[1]
   apply (intro conjI impI allI)
-     apply (simp add: s0_ptr_defs)
     apply clarsimp
     apply (drule not_disjointI,
              rule irq_node_offs_in_range,
@@ -1680,7 +1805,6 @@ lemma map_to_ctes_kh0H_simps[simp]:
            erule notE,
            rule kh0H_dom_sets_distinct)
    apply (clarsimp simp: kh0H_dom_distinct)
-  apply clarsimp
   apply (drule not_disjointI,
            rule irq_node_offs_in_range,
           assumption,
@@ -1693,7 +1817,6 @@ lemma map_to_ctes_kh0H_simps[simp]:
   apply ((simp add: offs_in_range kh0H_dom_sets_distinct[THEN orthD1] not_in_range_cte_None
         | simp add: offs_in_range kh0H_dom_sets_distinct[THEN orthD2] not_in_range_cte_None)+)[1]
   apply (intro conjI impI allI)
-     apply (simp add: s0_ptr_defs)
     apply clarsimp
     apply (drule not_disjointI,
              rule irq_node_offs_in_range,
@@ -1701,7 +1824,6 @@ lemma map_to_ctes_kh0H_simps[simp]:
            erule notE,
            rule kh0H_dom_sets_distinct)
    apply (clarsimp simp: kh0H_dom_distinct)
-  apply clarsimp
   apply (drule not_disjointI,
            rule irq_node_offs_in_range,
           assumption,
@@ -1714,7 +1836,6 @@ lemma map_to_ctes_kh0H_simps[simp]:
   apply ((simp add: offs_in_range kh0H_dom_sets_distinct[THEN orthD1] not_in_range_cte_None
         | simp add: offs_in_range kh0H_dom_sets_distinct[THEN orthD2] not_in_range_cte_None)+)[1]
   apply (intro conjI impI allI)
-     apply (simp add: s0_ptr_defs)
     apply clarsimp
     apply (drule not_disjointI,
              rule irq_node_offs_in_range,
@@ -1722,7 +1843,6 @@ lemma map_to_ctes_kh0H_simps[simp]:
            erule notE,
            rule kh0H_dom_sets_distinct)
    apply (clarsimp simp: kh0H_dom_distinct)
-  apply clarsimp
   apply (drule not_disjointI,
            rule irq_node_offs_in_range,
           assumption,
@@ -1735,7 +1855,6 @@ lemma map_to_ctes_kh0H_simps[simp]:
   apply ((simp add: offs_in_range kh0H_dom_sets_distinct[THEN orthD1] not_in_range_cte_None
         | simp add: offs_in_range kh0H_dom_sets_distinct[THEN orthD2] not_in_range_cte_None)+)[1]
   apply (intro conjI impI allI)
-     apply (simp add: s0_ptr_defs)
     apply clarsimp
     apply (drule not_disjointI,
              rule irq_node_offs_in_range,
@@ -1743,7 +1862,6 @@ lemma map_to_ctes_kh0H_simps[simp]:
            erule notE,
            rule kh0H_dom_sets_distinct)
    apply (clarsimp simp: kh0H_dom_distinct)
-  apply clarsimp
   apply (drule not_disjointI,
            rule irq_node_offs_in_range,
           assumption,
@@ -1757,7 +1875,6 @@ lemma map_to_ctes_kh0H_simps[simp]:
   apply ((simp add: offs_in_range kh0H_dom_sets_distinct[THEN orthD1] not_in_range_cte_None
         | simp add: offs_in_range kh0H_dom_sets_distinct[THEN orthD2] not_in_range_cte_None)+)[1]
   apply (intro conjI impI allI)
-     apply (simp add: s0_ptr_defs)
     apply clarsimp
     apply (drule not_disjointI,
              rule irq_node_offs_in_range,
@@ -1765,7 +1882,6 @@ lemma map_to_ctes_kh0H_simps[simp]:
            erule notE,
            rule kh0H_dom_sets_distinct)
    apply (clarsimp simp: kh0H_dom_distinct)
-  apply clarsimp
   apply (drule not_disjointI,
            rule irq_node_offs_in_range,
           assumption,
@@ -1778,7 +1894,6 @@ lemma map_to_ctes_kh0H_simps[simp]:
   apply ((simp add: offs_in_range kh0H_dom_sets_distinct[THEN orthD1] not_in_range_cte_None
         | simp add: offs_in_range kh0H_dom_sets_distinct[THEN orthD2] not_in_range_cte_None)+)[1]
   apply (intro conjI impI allI)
-     apply (simp add: s0_ptr_defs)
     apply clarsimp
     apply (drule not_disjointI,
              rule irq_node_offs_in_range,
@@ -1786,7 +1901,6 @@ lemma map_to_ctes_kh0H_simps[simp]:
            erule notE,
            rule kh0H_dom_sets_distinct)
    apply (clarsimp simp: kh0H_dom_distinct)
-  apply clarsimp
   apply (drule not_disjointI,
            rule irq_node_offs_in_range,
           assumption,
@@ -1799,7 +1913,6 @@ lemma map_to_ctes_kh0H_simps[simp]:
   apply ((simp add: offs_in_range kh0H_dom_sets_distinct[THEN orthD1] not_in_range_cte_None
         | simp add: offs_in_range kh0H_dom_sets_distinct[THEN orthD2] not_in_range_cte_None)+)[1]
   apply (intro conjI impI allI)
-     apply (simp add: s0_ptr_defs)
     apply clarsimp
     apply (drule not_disjointI,
              rule irq_node_offs_in_range,
@@ -1807,7 +1920,6 @@ lemma map_to_ctes_kh0H_simps[simp]:
            erule notE,
            rule kh0H_dom_sets_distinct)
    apply (clarsimp simp: kh0H_dom_distinct)
-  apply clarsimp
   apply (drule not_disjointI,
            rule irq_node_offs_in_range,
           assumption,
@@ -1820,7 +1932,6 @@ lemma map_to_ctes_kh0H_simps[simp]:
   apply ((simp add: offs_in_range kh0H_dom_sets_distinct[THEN orthD1] not_in_range_cte_None
         | simp add: offs_in_range kh0H_dom_sets_distinct[THEN orthD2] not_in_range_cte_None)+)[1]
   apply (intro conjI impI allI)
-     apply (simp add: s0_ptr_defs)
     apply clarsimp
     apply (drule not_disjointI,
              rule irq_node_offs_in_range,
@@ -1828,7 +1939,6 @@ lemma map_to_ctes_kh0H_simps[simp]:
            erule notE,
            rule kh0H_dom_sets_distinct)
    apply (clarsimp simp: kh0H_dom_distinct)
-  apply clarsimp
   by (drule not_disjointI,
         rule irq_node_offs_in_range,
        assumption,
@@ -1841,8 +1951,7 @@ lemma map_to_ctes_kh0H_dom:
                              Low_tcb_ptr, Low_tcb_ptr + 0x20, Low_tcb_ptr + 0x40,
                              Low_tcb_ptr + 0x60, Low_tcb_ptr + 0x80,
                              High_tcb_ptr, High_tcb_ptr + 0x20, High_tcb_ptr + 0x40,
-                             High_tcb_ptr + 0x60, High_tcb_ptr + 0x80,
-                             irq_cnode_ptr}
+                             High_tcb_ptr + 0x60, High_tcb_ptr + 0x80}
                            \<union> irq_node_offs_range
                            \<union> cnode_offs_range Silc_cnode_ptr
                            \<union> cnode_offs_range High_cnode_ptr
@@ -1897,8 +2006,7 @@ lemma map_to_ctes_kh0H_SomeD:
        x = High_tcb_ptr + 0x40 \<and> y = (CTE (ReplyCap High_tcb_ptr True True) (MDB 0 0 True True)) \<or>
        x = High_tcb_ptr + 0x60 \<and> y = (CTE NullCap Null_mdb) \<or>
        x = High_tcb_ptr + 0x80 \<and> y = (CTE NullCap Null_mdb) \<or>
-       x = irq_cnode_ptr \<and> y = (CTE NullCap Null_mdb) \<or>
-       x \<in> irq_node_offs_range \<and> y = (CTE NullCap Null_mdb) \<or>
+       x \<in> irq_node_offs_range \<and> y = irq_cte \<or>
        x \<in> cnode_offs_range Silc_cnode_ptr \<and> Silc_cte_cte Silc_cnode_ptr x \<noteq> None
                                            \<and> y = the (Silc_cte_cte Silc_cnode_ptr x) \<or>
        x \<in> cnode_offs_range High_cnode_ptr \<and> High_cte_cte High_cnode_ptr x \<noteq> None \<and> y = the (High_cte_cte High_cnode_ptr x) \<or>
@@ -1920,303 +2028,6 @@ lemma mask_neg_add_aligned:
 lemma mask_neg_add_aligned':
   "is_aligned q n \<Longrightarrow> q + p && ~~ mask n = (p && ~~ mask n) + q"
   by (simp add: mask_out_add_aligned[symmetric])
-
-lemma kh_s0H[simp]:
-  "ksPSpace s0H_internal = kh0H"
-  by (simp add: s0H_internal_def)
-
-lemma pspace_distinct'_split:
-  notes less_1_simp[simp del] shows
-  "(\<forall>(y, ko) \<in> graph_of (ksPSpace ks). (x \<le> y \<or> y + (1 << objBitsKO ko) - 1 < x)
-                                     \<and> y \<le> y + (1 << objBitsKO ko) - 1)
-   \<Longrightarrow> pspace_distinct' (ks \<lparr>ksPSpace := restrict_map (ksPSpace ks) {..< x}\<rparr>)
-   \<Longrightarrow> pspace_distinct' (ks \<lparr>ksPSpace := restrict_map (ksPSpace ks) {x ..}\<rparr>)
-   \<Longrightarrow> pspace_distinct' ks"
-  apply (clarsimp simp: pspace_distinct'_def)
-  apply (drule bspec, erule graph_ofI, clarsimp)
-  apply (simp add: Ball_def)
-  apply (drule_tac x=xa in spec)+
-  apply (erule disjE)
-   apply (simp add: domI)
-   apply (thin_tac "P \<longrightarrow> Q" for P Q)
-   apply (simp add: ps_clear_def)
-   apply (erule trans[rotated])
-   apply auto[1]
-  apply (clarsimp simp add: domI)
-  apply (drule mp, erule(1) order_le_less_trans)
-  apply (thin_tac "P \<longrightarrow> Q" for P Q)
-  apply (simp add: ps_clear_def)
-  apply (erule trans[rotated])
-  apply (fastforce simp: mask_eq_exp_minus_1 add_diff_eq)
-  done
-
-lemma irq_node_offs_range_def2:
-  "irq_node_offs_range = {x. init_irq_node_ptr \<le> x \<and> x \<le> init_irq_node_ptr + 0x7E0} \<inter>
-                         {x. is_aligned x 5}"
-  apply (safe, simp_all add: irq_node_offs_range_def add.commute)
-  by (auto dest: word_less_sub_1 simp: s0_ptr_defs elim: dual_order.strict_trans2[rotated])
-
-(* FIXME IF: fix repetitiveness *)
-lemma s0H_pspace_distinct':
-  notes pteBits_def[simp] objBits_defs[simp]
-  shows "pspace_distinct' s0H_internal"
-  supply option.case_cong[cong] if_cong[cong]
-  apply (clarsimp simp: pspace_distinct'_def ps_clear_def mask_eq_exp_minus_1)
-  apply (rule disjointI)
-  apply clarsimp
-  apply (drule kh0H_SomeD)+
-  \<comment> \<open>ntfn_ptr\<close>
-  apply (erule_tac P="_ \<and> y = _" in disjE)
-  subgoal by ((elim disjE; clarsimp),
-              (thin_tac "_ \<le> _", clarsimp simp: pt_offs_range_def page_offs_range_def
-                                                 cnode_offs_range_def irq_node_offs_range_def2
-                               , drule dual_order.trans, assumption
-                               , clarsimp simp: s0_ptr_defs objBitsKO_def
-               | solves \<open>clarsimp simp: s0_ptr_defs objBitsKO_def\<close>)+)
-  \<comment> \<open>Low_tcb_ptr\<close>
-  apply (erule_tac P="_ \<and> y = _" in disjE)
-  subgoal by ((elim disjE; clarsimp),
-              (thin_tac "_ \<le> _", clarsimp simp: pt_offs_range_def page_offs_range_def
-                                                 cnode_offs_range_def irq_node_offs_range_def2
-                               , drule dual_order.trans, assumption
-                               , clarsimp simp: s0_ptr_defs objBitsKO_def
-               | solves \<open>clarsimp simp: s0_ptr_defs objBitsKO_def\<close>)+)
-  \<comment> \<open>High_tcb_ptr\<close>
-  apply (erule_tac P="_ \<and> y = _" in disjE)
-  subgoal by ((elim disjE; clarsimp),
-              (thin_tac "_ \<le> _", clarsimp simp: pt_offs_range_def page_offs_range_def
-                                                 cnode_offs_range_def irq_node_offs_range_def2
-                               , drule dual_order.trans, assumption
-                               , clarsimp simp: s0_ptr_defs objBitsKO_def
-               | solves \<open>clarsimp simp: s0_ptr_defs objBitsKO_def\<close>)+)
-  \<comment> \<open>Idle_tcb_ptr\<close>
-  apply (erule_tac P="_ \<and> y = _" in disjE)
-  subgoal by ((elim disjE; clarsimp),
-              (thin_tac "_ \<le> _", clarsimp simp: pt_offs_range_def page_offs_range_def
-                                                 cnode_offs_range_def irq_node_offs_range_def2
-                               , drule dual_order.trans, assumption
-                               , clarsimp simp: s0_ptr_defs objBitsKO_def
-               | solves \<open>clarsimp simp: s0_ptr_defs objBitsKO_def\<close>)+)
-  \<comment> \<open>riscv_global_pt_ptr\<close>
-  apply (erule_tac P="_ \<and> _ \<and> y = _" in disjE)
-   apply (elim disjE; clarsimp)
-                   apply ((clarsimp simp: irq_node_offs_range_def2 pt_offs_range_def objBitsKO_def,
-                           drule dual_order.trans, assumption,
-                           (thin_tac "ya \<le> _", thin_tac "_ \<le> ya",
-                            drule_tac b=ya and a="_ + _" in dual_order.trans, assumption)?,
-                           simp add: s0_ptr_defs)+)[4]
-             apply (clarsimp simp: pt_offs_range_def objBitsKO_def archObjSize_def kh0H_obj_def bit_simps
-                            split: if_split_asm;
-                    (drule (1) aligned_le_sharp, simp add: mask_neg_add_aligned', fastforce simp: mask_def))
-             apply (thin_tac "_ \<le> _",
-                    clarsimp simp: kh0H_obj_def objBitsKO_def archObjSize_def bit_simps pt_offs_range_def
-                                   irq_node_offs_range_def2 cnode_offs_range_def page_offs_range_def,
-                    drule_tac a=x and b="_ + _" in aligned_le_sharp, assumption,
-                    drule dual_order.trans[rotated],
-                    erule word_plus_mono_left, simp add: s0_ptr_defs mask_def,
-                    (drule_tac b=ya and a="(_ && ~~ mask _) + _" in dual_order.trans, assumption)?,
-                    simp add: s0_ptr_defs mask_def)+
-  \<comment> \<open>irq_node_offs_range\<close>
-  apply (erule_tac P="_ \<and> y = _" in disjE)
-   apply (elim disjE; clarsimp)
-                   apply ((clarsimp simp: irq_node_offs_range_def2 pt_offs_range_def objBitsKO_def,
-                           drule dual_order.trans, assumption,
-                           (thin_tac "ya \<le> _", thin_tac "_ \<le> ya",
-                            drule_tac b=ya and a="_ + _" in dual_order.trans, assumption)?,
-                           simp add: s0_ptr_defs)+)[5]
-              apply (clarsimp simp: irq_node_offs_range_def objBitsKO_def archObjSize_def kh0H_obj_def
-                             split: if_split_asm;
-                     (drule(1) aligned_le_sharp, simp add: mask_neg_add_aligned', fastforce simp: mask_def))
-             apply (thin_tac "_ \<le> _",
-                    clarsimp simp: kh0H_obj_def objBitsKO_def archObjSize_def bit_simps pt_offs_range_def
-                                   irq_node_offs_range_def2 cnode_offs_range_def page_offs_range_def,
-                    drule_tac a=x and b="_ + _" in aligned_le_sharp, assumption,
-                    drule dual_order.trans[rotated],
-                    erule word_plus_mono_left, simp add: s0_ptr_defs mask_def,
-                    (drule_tac b=ya and a="(_ && ~~ mask _) + _" in dual_order.trans, assumption)?,
-                    simp add: s0_ptr_defs mask_def)+
-  \<comment> \<open>Low_pt_ptr\<close>
-  apply (erule_tac P="_ \<and> _ \<and> y = _" in disjE)
-   apply (elim disjE; clarsimp)
-                   apply ((clarsimp simp: irq_node_offs_range_def2 pt_offs_range_def objBitsKO_def,
-                           drule dual_order.trans, assumption,
-                           (thin_tac "ya \<le> _", thin_tac "_ \<le> ya",
-                            drule_tac b=ya and a="_ + _" in dual_order.trans, assumption)?,
-                           simp add: s0_ptr_defs)+)[6]
-             apply (clarsimp simp: pt_offs_range_def objBitsKO_def archObjSize_def kh0H_obj_def bit_simps
-                            split: if_split_asm;
-                    (drule (1) aligned_le_sharp, simp add: mask_neg_add_aligned', fastforce simp: mask_def))
-             apply (thin_tac "_ \<le> _",
-                    clarsimp simp: kh0H_obj_def objBitsKO_def archObjSize_def bit_simps pt_offs_range_def
-                                   irq_node_offs_range_def2 cnode_offs_range_def page_offs_range_def,
-                    drule_tac a=x and b="_ + _" in aligned_le_sharp, assumption,
-                    drule dual_order.trans[rotated],
-                    erule word_plus_mono_left, simp add: s0_ptr_defs mask_def,
-                    (drule_tac b=ya and a="(_ && ~~ mask _) + _" in dual_order.trans, assumption)?,
-                    simp add: s0_ptr_defs mask_def)+
-  \<comment> \<open>High_pt_ptr\<close>
-  apply (erule_tac P="_ \<and> _ \<and> y = _" in disjE)
-   apply (elim disjE; clarsimp)
-                   apply ((clarsimp simp: irq_node_offs_range_def2 pt_offs_range_def objBitsKO_def,
-                           drule dual_order.trans, assumption,
-                           (thin_tac "ya \<le> _", thin_tac "_ \<le> ya",
-                            drule_tac b=ya and a="_ + _" in dual_order.trans, assumption)?,
-                           simp add: s0_ptr_defs)+)[7]
-             apply (clarsimp simp: pt_offs_range_def objBitsKO_def archObjSize_def kh0H_obj_def bit_simps
-                            split: if_split_asm;
-                    (drule (1) aligned_le_sharp, simp add: mask_neg_add_aligned', fastforce simp: mask_def))
-             apply (thin_tac "_ \<le> _",
-                    clarsimp simp: kh0H_obj_def objBitsKO_def archObjSize_def bit_simps pt_offs_range_def
-                                   irq_node_offs_range_def2 cnode_offs_range_def page_offs_range_def,
-                    drule_tac a=x and b="_ + _" in aligned_le_sharp, assumption,
-                    drule dual_order.trans[rotated],
-                    erule word_plus_mono_left, simp add: s0_ptr_defs mask_def,
-                    (drule_tac b=ya and a="(_ && ~~ mask _) + _" in dual_order.trans, assumption)?,
-                    simp add: s0_ptr_defs mask_def)+
-  \<comment> \<open>Low_pd_ptr\<close>
-  apply (erule_tac P="_ \<and> _ \<and> y = _" in disjE)
-   apply (elim disjE; clarsimp)
-                   apply ((clarsimp simp: irq_node_offs_range_def2 pt_offs_range_def objBitsKO_def,
-                           drule dual_order.trans, assumption,
-                           (thin_tac "ya \<le> _", thin_tac "_ \<le> ya",
-                            drule_tac b=ya and a="_ + _" in dual_order.trans, assumption)?,
-                           simp add: s0_ptr_defs)+)[8]
-             apply (clarsimp simp: pt_offs_range_def objBitsKO_def archObjSize_def kh0H_obj_def bit_simps
-                            split: if_split_asm;
-                    (drule (1) aligned_le_sharp, simp add: mask_neg_add_aligned', fastforce simp: mask_def))
-             apply (thin_tac "_ \<le> _",
-                    clarsimp simp: kh0H_obj_def objBitsKO_def archObjSize_def bit_simps pt_offs_range_def
-                                   irq_node_offs_range_def2 cnode_offs_range_def page_offs_range_def,
-                    drule_tac a=x and b="_ + _" in aligned_le_sharp, assumption,
-                    drule dual_order.trans[rotated],
-                    erule word_plus_mono_left, simp add: s0_ptr_defs mask_def,
-                    (drule_tac b=ya and a="(_ && ~~ mask _) + _" in dual_order.trans, assumption)?,
-                    simp add: s0_ptr_defs mask_def)+
-  \<comment> \<open>High_pd_ptr\<close>
-  apply (erule_tac P="_ \<and> _ \<and> y = _" in disjE)
-   apply (elim disjE; clarsimp)
-                   apply ((clarsimp simp: irq_node_offs_range_def2 pt_offs_range_def objBitsKO_def,
-                           drule dual_order.trans, assumption,
-                           (thin_tac "ya \<le> _", thin_tac "_ \<le> ya",
-                            drule_tac b=ya and a="_ + _" in dual_order.trans, assumption)?,
-                           simp add: s0_ptr_defs)+)[9]
-             apply (clarsimp simp: pt_offs_range_def objBitsKO_def archObjSize_def kh0H_obj_def bit_simps
-                            split: if_split_asm;
-                    (drule (1) aligned_le_sharp, simp add: mask_neg_add_aligned', fastforce simp: mask_def))
-             apply (thin_tac "_ \<le> _",
-                    clarsimp simp: kh0H_obj_def objBitsKO_def archObjSize_def bit_simps pt_offs_range_def
-                                   irq_node_offs_range_def cnode_offs_range_def page_offs_range_def,
-                    drule_tac a=x and b="_ + _" in aligned_le_sharp, assumption,
-                    drule dual_order.trans[rotated],
-                    erule word_plus_mono_left, simp add: s0_ptr_defs mask_def,
-                    (drule_tac b=ya and a="(_ && ~~ mask _) + _" in dual_order.trans, assumption)?,
-                    simp add: s0_ptr_defs mask_def)+
-  \<comment> \<open>Low_pool_ptr\<close>
-  apply (erule_tac P="_ \<and> y = _" in disjE)
-   subgoal for x y ya yb
-   by ((elim disjE; clarsimp),
-       ((clarsimp simp: irq_node_offs_range_def2 pt_offs_range_def cnode_offs_range_def
-                        page_offs_range_def objBitsKO_def archObjSize_def kh0H_obj_def,
-         (thin_tac "ya \<le> _", drule dual_order.trans, assumption |
-          thin_tac "_ \<le> ya", drule dual_order.trans, assumption)?,
-         solves \<open>clarsimp simp: s0_ptr_defs bit_simps\<close>)+))
-  \<comment> \<open>High_pool_ptr\<close>
-  apply (erule_tac P="_ \<and> y = _" in disjE)
-   subgoal for x y ya yb
-   by ((elim disjE; clarsimp),
-       ((clarsimp simp: irq_node_offs_range_def2 pt_offs_range_def cnode_offs_range_def
-                        page_offs_range_def objBitsKO_def archObjSize_def kh0H_obj_def,
-         (thin_tac "ya \<le> _", drule dual_order.trans, assumption |
-          thin_tac "_ \<le> ya", drule dual_order.trans, assumption)?,
-         solves \<open>clarsimp simp: s0_ptr_defs bit_simps\<close>)+))
-  \<comment> \<open>Low_cnode_ptr\<close>
-  apply (erule_tac P="_ \<and> _ \<and> y = _" in disjE)
-  apply (elim disjE; clarsimp)
-                  apply ((clarsimp simp: cnode_offs_range_def irq_node_offs_range_def2
-                                         pt_offs_range_def objBitsKO_def,
-                          drule dual_order.trans, assumption,
-                          (thin_tac "ya \<le> _", thin_tac "_ \<le> ya",
-                           drule_tac b=ya and a="_ + _" in dual_order.trans, assumption)?,
-                          simp add: s0_ptr_defs)+)[12]
-      apply (clarsimp simp: objBitsKO_def kh0H_obj_def Low_cte'_def Low_capsH_def cnode_offs_range_def
-                     split: if_split_asm;
-             (drule (1) aligned_le_sharp, simp add: mask_neg_add_aligned', fastforce simp: mask_def))
-             apply (thin_tac "_ \<le> _",
-                    clarsimp simp: kh0H_obj_def objBitsKO_def archObjSize_def bit_simps pt_offs_range_def
-                                   irq_node_offs_range_def cnode_offs_range_def page_offs_range_def,
-                    drule_tac a=x and b="_ + _" in aligned_le_sharp, assumption,
-                    drule dual_order.trans[rotated],
-                    erule word_plus_mono_left, simp add: s0_ptr_defs mask_def,
-                    (drule_tac b=ya and a="(_ && ~~ mask _) + _" in dual_order.trans, assumption)?,
-                    simp add: s0_ptr_defs mask_def)+
-  \<comment> \<open>High_cnode_ptr\<close>
-  apply (erule_tac P="_ \<and> _ \<and> y = _" in disjE)
-  apply (elim disjE; clarsimp)
-                  apply ((clarsimp simp: cnode_offs_range_def irq_node_offs_range_def2
-                                         pt_offs_range_def objBitsKO_def,
-                          drule dual_order.trans, assumption,
-                          (thin_tac "ya \<le> _", thin_tac "_ \<le> ya",
-                           drule_tac b=ya and a="_ + _" in dual_order.trans, assumption)?,
-                          simp add: s0_ptr_defs)+)[13]
-      apply (clarsimp simp: objBitsKO_def kh0H_obj_def High_cte'_def High_capsH_def cnode_offs_range_def
-                     split: if_split_asm;
-             (drule (1) aligned_le_sharp, simp add: mask_neg_add_aligned', fastforce simp: mask_def))
-             apply (thin_tac "_ \<le> _",
-                    clarsimp simp: kh0H_obj_def objBitsKO_def archObjSize_def bit_simps pt_offs_range_def
-                                   irq_node_offs_range_def cnode_offs_range_def page_offs_range_def,
-                    drule_tac a=x and b="_ + _" in aligned_le_sharp, assumption,
-                    drule dual_order.trans[rotated],
-                    erule word_plus_mono_left, simp add: s0_ptr_defs mask_def,
-                    (drule_tac b=ya and a="(_ && ~~ mask _) + _" in dual_order.trans, assumption)?,
-                    simp add: s0_ptr_defs mask_def)+
-  \<comment> \<open>Silc_cnode_ptr\<close>
-  apply (erule_tac P="_ \<and> _ \<and> y = _" in disjE)
-  apply (elim disjE; clarsimp)
-                  apply ((clarsimp simp: cnode_offs_range_def irq_node_offs_range_def2
-                                         pt_offs_range_def objBitsKO_def,
-                          drule dual_order.trans, assumption,
-                          (thin_tac "ya \<le> _", thin_tac "_ \<le> ya",
-                           drule_tac b=ya and a="_ + _" in dual_order.trans, assumption)?,
-                          simp add: s0_ptr_defs)+)[14]
-      apply (clarsimp simp: objBitsKO_def kh0H_obj_def Silc_cte'_def Silc_capsH_def cnode_offs_range_def
-                     split: if_split_asm;
-             (drule (1) aligned_le_sharp, simp add: mask_neg_add_aligned', fastforce simp: mask_def))
-             apply (thin_tac "_ \<le> _",
-                    clarsimp simp: kh0H_obj_def objBitsKO_def archObjSize_def bit_simps pt_offs_range_def
-                                   irq_node_offs_range_def cnode_offs_range_def page_offs_range_def,
-                    drule_tac a=x and b="_ + _" in aligned_le_sharp, assumption,
-                    drule dual_order.trans[rotated],
-                    erule word_plus_mono_left, simp add: s0_ptr_defs mask_def,
-                    (drule_tac b=ya and a="(_ && ~~ mask _) + _" in dual_order.trans, assumption)?,
-                    simp add: s0_ptr_defs mask_def)+
-  \<comment> \<open>irq_cnode_ptr\<close>
-  apply (erule_tac P="_ \<and> y = _" in disjE)
-   subgoal for x y ya yb
-   by ((elim disjE; clarsimp),
-       ((clarsimp simp: irq_node_offs_range_def2 pt_offs_range_def cnode_offs_range_def
-                        page_offs_range_def objBitsKO_def archObjSize_def kh0H_obj_def,
-         (thin_tac "ya \<le> _", drule dual_order.trans, assumption |
-          thin_tac "_ \<le> ya", drule dual_order.trans, assumption)?,
-         solves \<open>clarsimp simp: s0_ptr_defs bit_simps\<close>)+))
-  \<comment> \<open>shared_page_ptr\<close>
-  apply (elim disjE; clarsimp)
-                 apply ((clarsimp simp: cnode_offs_range_def irq_node_offs_range_def2
-                                        page_offs_range_def pt_offs_range_def objBitsKO_def,
-                         drule dual_order.trans, assumption,
-                         (thin_tac "ya \<le> _", thin_tac "_ \<le> ya",
-                          drule_tac b=ya and a="_ + _" in dual_order.trans, assumption)?,
-                         simp add: s0_ptr_defs)+)[16]
-  apply (clarsimp simp: page_offs_range_def objBitsKO_def archObjSize_def bit_simps)
-  apply (drule (1) aligned_le_sharp, simp add: mask_neg_add_aligned', fastforce simp: mask_def)
-  done
-
-lemma pspace_distinctD'':
-  "\<lbrakk> \<exists>v. ksPSpace s x = Some v \<and> objBitsKO v = n; pspace_distinct' s \<rbrakk>
-     \<Longrightarrow> ps_clear x n s"
-  apply clarsimp
-  apply (drule(1) pspace_distinctD')
-  apply simp
-  done
 
 lemma cnode_offs_min2':
   "is_aligned ptr 15 \<Longrightarrow> (ptr :: obj_ref) \<le> ptr + 0x20 * (x && mask 10)"
@@ -2258,7 +2069,8 @@ lemma cnode_offs_max2:
 
 lemma cnode_offs_in_range2':
   "is_aligned ptr 15 \<Longrightarrow> ptr + 0x20 * (x && mask 10) \<in> cnode_offs_range ptr"
-  apply (clarsimp simp: cnode_offs_min2' cnode_offs_max2' cnode_offs_range_def add.commute)
+  apply (clarsimp simp: cnode_offs_min2' cnode_offs_max2' cnode_offs_range_def cte_level_bits_def
+                        add.commute)
   apply (rule is_aligned_add)
    apply (erule is_aligned_weaken)
    apply simp
@@ -2277,21 +2089,21 @@ lemma kh0H_dom_distinct2:
   "Silc_cnode_ptr + 0x20 * (x && mask 10) \<noteq> Low_tcb_ptr"
   "Silc_cnode_ptr + 0x20 * (x && mask 10) \<noteq> High_pool_ptr"
   "Silc_cnode_ptr + 0x20 * (x && mask 10) \<noteq> Low_pool_ptr"
-  "Silc_cnode_ptr + 0x20 * (x && mask 10) \<noteq> irq_cnode_ptr"
+  "Silc_cnode_ptr + 0x20 * (x && mask 10) \<noteq> init_irq_node_ptr"
   "Silc_cnode_ptr + 0x20 * (x && mask 10) \<noteq> ntfn_ptr"
   "Low_cnode_ptr + 0x20 * (x && mask 10) \<noteq> idle_tcb_ptr"
   "Low_cnode_ptr + 0x20 * (x && mask 10) \<noteq> High_tcb_ptr"
   "Low_cnode_ptr + 0x20 * (x && mask 10) \<noteq> Low_tcb_ptr"
   "Low_cnode_ptr + 0x20 * (x && mask 10) \<noteq> High_pool_ptr"
   "Low_cnode_ptr + 0x20 * (x && mask 10) \<noteq> Low_pool_ptr"
-  "Low_cnode_ptr + 0x20 * (x && mask 10) \<noteq> irq_cnode_ptr"
+  "Low_cnode_ptr + 0x20 * (x && mask 10) \<noteq> init_irq_node_ptr"
   "Low_cnode_ptr + 0x20 * (x && mask 10) \<noteq> ntfn_ptr"
   "High_cnode_ptr + 0x20 * (x && mask 10) \<noteq> idle_tcb_ptr"
   "High_cnode_ptr + 0x20 * (x && mask 10) \<noteq> High_tcb_ptr"
   "High_cnode_ptr + 0x20 * (x && mask 10) \<noteq> Low_tcb_ptr"
   "High_cnode_ptr + 0x20 * (x && mask 10) \<noteq> High_pool_ptr"
   "High_cnode_ptr + 0x20 * (x && mask 10) \<noteq> Low_pool_ptr"
-  "High_cnode_ptr + 0x20 * (x && mask 10) \<noteq> irq_cnode_ptr"
+  "High_cnode_ptr + 0x20 * (x && mask 10) \<noteq> init_irq_node_ptr"
   "High_cnode_ptr + 0x20 * (x && mask 10) \<noteq> ntfn_ptr"
   by (cut_tac x=x in cnode_offs_in_range2(1), fastforce simp: kh0H_dom_distinct
       | cut_tac x=x in cnode_offs_in_range2(2), fastforce simp: kh0H_dom_distinct
@@ -2339,6 +2151,14 @@ lemma less_0x200_exists_ucast:
   apply clarsimp
   done
 
+lemma pspace_distinctD'':
+  "\<lbrakk> \<exists>v. ksPSpace s x = Some v \<and> objBitsKO v = n; pspace_distinct' s \<rbrakk>
+     \<Longrightarrow> ps_clear x n s"
+  apply clarsimp
+  apply (drule(1) pspace_distinctD')
+  apply simp
+  done
+
 lemma valid_caps_s0H[simp]:
   notes pteBits_def[simp] objBits_defs[simp]
   shows
@@ -2361,13 +2181,27 @@ lemma valid_caps_s0H[simp]:
   "valid_cap' (NotificationCap ntfn_ptr 0 False True) s0H_internal"
   "valid_cap' (ReplyCap Low_tcb_ptr True True) s0H_internal"
   "valid_cap' (ReplyCap High_tcb_ptr True True) s0H_internal"
-  supply option.case_cong[cong] if_cong[cong]
+  supply option.case_cong[cong] if_cong[cong] cte_level_bits_def[simp]
   apply (simp | simp add: valid_cap'_def s0H_internal_def capAligned_def word_bits_def
                           objBits_def s0_ptrs_aligned obj_at'_def,
                 intro conjI, simp add: objBitsKO_def s0_ptrs_aligned, simp add: objBitsKO_def,
                 simp add: objBitsKO_def s0_ptrs_aligned mask_def,
                 rule pspace_distinctD'[OF _ s0H_pspace_distinct', simplified s0H_internal_def],
                 simp)+
+   apply (simp add: valid_cap'_def capAligned_def word_bits_def objBits_def s0_ptrs_aligned obj_at'_def)
+   apply (intro conjI)
+      apply (simp add: objBitsKO_def s0_ptrs_aligned)
+     apply (simp add: objBitsKO_def)
+    apply (simp add: objBitsKO_def s0_ptrs_aligned mask_def)
+   apply (rule pspace_distinctD''[OF _ s0H_pspace_distinct'])
+   apply clarsimp
+   apply (simp add: valid_cap'_def capAligned_def word_bits_def objBits_def s0_ptrs_aligned obj_at'_def)
+   apply (intro conjI)
+      apply (simp add: objBitsKO_def s0_ptrs_aligned)
+     apply (simp add: objBitsKO_def)
+    apply (simp add: objBitsKO_def s0_ptrs_aligned mask_def)
+   apply (rule pspace_distinctD''[OF _ s0H_pspace_distinct'])
+   apply clarsimp
    apply (simp add: valid_cap'_def capAligned_def word_bits_def objBits_def s0_ptrs_aligned obj_at'_def)
    apply (intro conjI)
       apply (simp add: objBitsKO_def s0_ptrs_aligned)
@@ -2424,7 +2258,9 @@ lemma valid_caps_s0H[simp]:
   by (simp add: valid_cap'_def s0H_internal_def capAligned_def word_bits_def objBits_def obj_at'_def,
       intro conjI, simp add: objBitsKO_def s0_ptrs_aligned, simp add: objBitsKO_def,
       simp add: objBitsKO_def s0_ptrs_aligned mask_def,
-      rule pspace_distinctD'[OF _ s0H_pspace_distinct', simplified s0H_internal_def], simp)+
+      rule pspace_distinctD'[OF _ s0H_pspace_distinct',
+                             simplified s0H_internal_def cte_level_bits_def],
+      simp)+
 
 text \<open>We can only instantiate our example state (featuring high and low domains) if the number
   of configured domains is > 1, i.e. that maxDomain is 1 or greater. When seL4 is configured for a
@@ -2674,39 +2510,40 @@ lemma map_to_ctes_kh0H_simps'[simp]:
                                                         (MDB (Low_cnode_ptr + 0xA0) (High_cnode_ptr + 0xA0) False False))"
   "map_to_ctes kh0H (Silc_cnode_ptr + 0x27C0) = Some (CTE (NotificationCap ntfn_ptr 0 True False)
                                                           (MDB (High_cnode_ptr + 318 * 0x20) (Low_cnode_ptr + 318 * 0x20) False False))"
-                  apply (clarsimp simp: map_to_ctes_kh0H_simps(3)[where x="the_nat_to_bl_10 1", simplified the_nat_to_bl_simps, simplified]
+    supply cte_level_bits_def[simp]
+                  apply (clarsimp simp: map_to_ctes_kh0H_simps(2)[where x="the_nat_to_bl_10 1", simplified the_nat_to_bl_simps, simplified]
                                         kh0H_all_obj_def' to_bl_use_of_bl the_nat_to_bl_simps, fastforce simp: s0_ptr_defs is_aligned_def)
-                 apply (clarsimp simp: map_to_ctes_kh0H_simps(3)[where x="the_nat_to_bl_10 2", simplified the_nat_to_bl_simps, simplified]
+                 apply (clarsimp simp: map_to_ctes_kh0H_simps(2)[where x="the_nat_to_bl_10 2", simplified the_nat_to_bl_simps, simplified]
                                        kh0H_all_obj_def' to_bl_use_of_bl the_nat_to_bl_simps, fastforce simp: s0_ptr_defs is_aligned_def)
-                apply (clarsimp simp: map_to_ctes_kh0H_simps(3)[where x="the_nat_to_bl_10 3", simplified the_nat_to_bl_simps, simplified]
+                apply (clarsimp simp: map_to_ctes_kh0H_simps(2)[where x="the_nat_to_bl_10 3", simplified the_nat_to_bl_simps, simplified]
                                       kh0H_all_obj_def' to_bl_use_of_bl the_nat_to_bl_simps, fastforce simp: s0_ptr_defs is_aligned_def)
-               apply (clarsimp simp: map_to_ctes_kh0H_simps(3)[where x="the_nat_to_bl_10 4", simplified the_nat_to_bl_simps, simplified]
+               apply (clarsimp simp: map_to_ctes_kh0H_simps(2)[where x="the_nat_to_bl_10 4", simplified the_nat_to_bl_simps, simplified]
                                      kh0H_all_obj_def' to_bl_use_of_bl the_nat_to_bl_simps, fastforce simp: s0_ptr_defs is_aligned_def)
-              apply (clarsimp simp: map_to_ctes_kh0H_simps(3)[where x="the_nat_to_bl_10 5", simplified the_nat_to_bl_simps, simplified]
+              apply (clarsimp simp: map_to_ctes_kh0H_simps(2)[where x="the_nat_to_bl_10 5", simplified the_nat_to_bl_simps, simplified]
                                     kh0H_all_obj_def' to_bl_use_of_bl the_nat_to_bl_simps, fastforce simp: s0_ptr_defs is_aligned_def)
-             apply (clarsimp simp: map_to_ctes_kh0H_simps(3)[where x="the_nat_to_bl_10 6", simplified the_nat_to_bl_simps, simplified]
+             apply (clarsimp simp: map_to_ctes_kh0H_simps(2)[where x="the_nat_to_bl_10 6", simplified the_nat_to_bl_simps, simplified]
                                    kh0H_all_obj_def' to_bl_use_of_bl the_nat_to_bl_simps, fastforce simp: s0_ptr_defs is_aligned_def)
-            apply (clarsimp simp: map_to_ctes_kh0H_simps(3)[where x="the_nat_to_bl_10 318", simplified the_nat_to_bl_simps, simplified]
+            apply (clarsimp simp: map_to_ctes_kh0H_simps(2)[where x="the_nat_to_bl_10 318", simplified the_nat_to_bl_simps, simplified]
                                   kh0H_all_obj_def' to_bl_use_of_bl the_nat_to_bl_simps, fastforce simp: s0_ptr_defs is_aligned_def)
-           apply (clarsimp simp: map_to_ctes_kh0H_simps(4)[where x="the_nat_to_bl_10 1", simplified the_nat_to_bl_simps, simplified]
+           apply (clarsimp simp: map_to_ctes_kh0H_simps(3)[where x="the_nat_to_bl_10 1", simplified the_nat_to_bl_simps, simplified]
                                  kh0H_all_obj_def' to_bl_use_of_bl the_nat_to_bl_simps, fastforce simp: s0_ptr_defs is_aligned_def)
-          apply (clarsimp simp: map_to_ctes_kh0H_simps(4)[where x="the_nat_to_bl_10 2", simplified the_nat_to_bl_simps, simplified]
+          apply (clarsimp simp: map_to_ctes_kh0H_simps(3)[where x="the_nat_to_bl_10 2", simplified the_nat_to_bl_simps, simplified]
                                 kh0H_all_obj_def' to_bl_use_of_bl the_nat_to_bl_simps, fastforce simp: s0_ptr_defs is_aligned_def)
-         apply (clarsimp simp: map_to_ctes_kh0H_simps(4)[where x="the_nat_to_bl_10 3", simplified the_nat_to_bl_simps, simplified]
+         apply (clarsimp simp: map_to_ctes_kh0H_simps(3)[where x="the_nat_to_bl_10 3", simplified the_nat_to_bl_simps, simplified]
                                kh0H_all_obj_def' to_bl_use_of_bl the_nat_to_bl_simps, fastforce simp: s0_ptr_defs is_aligned_def)
-        apply (clarsimp simp: map_to_ctes_kh0H_simps(4)[where x="the_nat_to_bl_10 4", simplified the_nat_to_bl_simps, simplified]
+        apply (clarsimp simp: map_to_ctes_kh0H_simps(3)[where x="the_nat_to_bl_10 4", simplified the_nat_to_bl_simps, simplified]
                               kh0H_all_obj_def' to_bl_use_of_bl the_nat_to_bl_simps, fastforce simp: s0_ptr_defs is_aligned_def)
-       apply (clarsimp simp: map_to_ctes_kh0H_simps(4)[where x="the_nat_to_bl_10 5", simplified the_nat_to_bl_simps, simplified]
+       apply (clarsimp simp: map_to_ctes_kh0H_simps(3)[where x="the_nat_to_bl_10 5", simplified the_nat_to_bl_simps, simplified]
                              kh0H_all_obj_def' to_bl_use_of_bl the_nat_to_bl_simps, fastforce simp: s0_ptr_defs is_aligned_def)
-      apply (clarsimp simp: map_to_ctes_kh0H_simps(4)[where x="the_nat_to_bl_10 6", simplified the_nat_to_bl_simps, simplified]
+      apply (clarsimp simp: map_to_ctes_kh0H_simps(3)[where x="the_nat_to_bl_10 6", simplified the_nat_to_bl_simps, simplified]
                             kh0H_all_obj_def' to_bl_use_of_bl the_nat_to_bl_simps, fastforce simp: s0_ptr_defs is_aligned_def)
-     apply (clarsimp simp: map_to_ctes_kh0H_simps(4)[where x="the_nat_to_bl_10 318", simplified the_nat_to_bl_simps, simplified]
+     apply (clarsimp simp: map_to_ctes_kh0H_simps(3)[where x="the_nat_to_bl_10 318", simplified the_nat_to_bl_simps, simplified]
                            kh0H_all_obj_def' to_bl_use_of_bl the_nat_to_bl_simps, fastforce simp: s0_ptr_defs is_aligned_def)
-    apply (clarsimp simp: map_to_ctes_kh0H_simps(5)[where x="the_nat_to_bl_10 2", simplified the_nat_to_bl_simps, simplified]
+    apply (clarsimp simp: map_to_ctes_kh0H_simps(4)[where x="the_nat_to_bl_10 2", simplified the_nat_to_bl_simps, simplified]
                           kh0H_all_obj_def' to_bl_use_of_bl the_nat_to_bl_simps, fastforce simp: s0_ptr_defs is_aligned_def)
-   apply (clarsimp simp: map_to_ctes_kh0H_simps(5)[where x="the_nat_to_bl_10 5", simplified the_nat_to_bl_simps, simplified]
+   apply (clarsimp simp: map_to_ctes_kh0H_simps(4)[where x="the_nat_to_bl_10 5", simplified the_nat_to_bl_simps, simplified]
                          kh0H_all_obj_def' to_bl_use_of_bl the_nat_to_bl_simps, fastforce simp: s0_ptr_defs is_aligned_def)
-  apply (clarsimp simp: map_to_ctes_kh0H_simps(5)[where x="the_nat_to_bl_10 318", simplified the_nat_to_bl_simps, simplified]
+  apply (clarsimp simp: map_to_ctes_kh0H_simps(4)[where x="the_nat_to_bl_10 318", simplified the_nat_to_bl_simps, simplified]
                         kh0H_all_obj_def' to_bl_use_of_bl the_nat_to_bl_simps, fastforce simp: s0_ptr_defs is_aligned_def)
   done
 
@@ -2726,17 +2563,20 @@ lemma mdb_next_s0H:
    apply (elim exE conjE)
    apply (frule map_to_ctes_kh0H_SomeD)
    apply (elim disjE, simp_all)[1]
+      apply (clarsimp simp: kh0H_all_obj_def' to_bl_use_of_bl the_nat_to_bl_simps
+                            ucast_shiftr_13E ucast_shiftr_5 s0_ptrs_aligned cte_level_bits_def
+                     split: if_split_asm)
      apply (clarsimp simp: kh0H_all_obj_def' to_bl_use_of_bl the_nat_to_bl_simps
-                           ucast_shiftr_13E ucast_shiftr_5 s0_ptrs_aligned
+                           ucast_shiftr_13E ucast_shiftr_5 s0_ptrs_aligned cte_level_bits_def
                     split: if_split_asm)
     apply (clarsimp simp: kh0H_all_obj_def' to_bl_use_of_bl the_nat_to_bl_simps
-                          ucast_shiftr_5 s0_ptrs_aligned
+                          ucast_shiftr_5 s0_ptrs_aligned cte_level_bits_def
                    split: if_split_asm)
    apply (clarsimp simp: kh0H_all_obj_def' to_bl_use_of_bl the_nat_to_bl_simps
-                         ucast_shiftr_13E ucast_shiftr_5 s0_ptrs_aligned
+                         ucast_shiftr_13E ucast_shiftr_5 s0_ptrs_aligned cte_level_bits_def
                   split: if_split_asm)
   apply (clarsimp simp: next_unfold' map_to_ctes_kh0H_dom)
-  apply (elim disjE, simp_all add: kh0H_all_obj_def')
+  apply (elim disjE, simp_all add: kh0H_all_obj_def')[1]
   done
 
 lemma mdb_prev_s0H:
@@ -2755,16 +2595,20 @@ lemma mdb_prev_s0H:
    apply (elim exE conjE)
    apply (frule map_to_ctes_kh0H_SomeD)
    apply (elim disjE, simp_all)[1]
+      apply clarsimp
+      apply (clarsimp simp: kh0H_all_obj_def' to_bl_use_of_bl the_nat_to_bl_simps
+                            ucast_shiftr_13E ucast_shiftr_5 s0_ptrs_aligned cte_level_bits_def
+                     split: if_split_asm)
      apply clarsimp
      apply (clarsimp simp: kh0H_all_obj_def' to_bl_use_of_bl the_nat_to_bl_simps
-                           ucast_shiftr_13E ucast_shiftr_5 s0_ptrs_aligned
+                           ucast_shiftr_13E ucast_shiftr_5 s0_ptrs_aligned cte_level_bits_def
                     split: if_split_asm)
     apply clarsimp
-    apply (clarsimp simp: kh0H_all_obj_def' to_bl_use_of_bl the_nat_to_bl_simps
+    apply (clarsimp simp: kh0H_all_obj_def' to_bl_use_of_bl the_nat_to_bl_simps cte_level_bits_def
                           ucast_shiftr_13E ucast_shiftr_3 ucast_shiftr_2 s0_ptrs_aligned
                    split: if_split_asm)
    apply clarsimp
-   apply (clarsimp simp: kh0H_all_obj_def' to_bl_use_of_bl the_nat_to_bl_simps
+   apply (clarsimp simp: kh0H_all_obj_def' to_bl_use_of_bl the_nat_to_bl_simps cte_level_bits_def
                          ucast_shiftr_5 ucast_shiftr_3 ucast_shiftr_2 s0_ptrs_aligned
                   split: if_split_asm)
   apply (clarsimp simp: mdb_prev_def map_to_ctes_kh0H_dom)
@@ -2784,6 +2628,7 @@ lemma mdb_next_trancl_s0H:
         p = Low_tcb_ptr + 0x20 \<and> p' = Low_cnode_ptr + 0x60 \<or>
         p = High_tcb_ptr \<and> p' = High_cnode_ptr + 0x40 \<or>
         p = High_tcb_ptr + 0x20 \<and> p' = High_cnode_ptr + 0x60)"
+  supply cte_level_bits_def[simp]
   apply (rule iffI)
    apply (erule converse_trancl_induct)
     apply (clarsimp simp: mdb_next_s0H)
@@ -2831,67 +2676,79 @@ lemma sameRegionAs_s0H:
           p = High_cnode_ptr + 0x40 \<and> p' = High_tcb_ptr \<or>
           p = High_tcb_ptr + 0x20 \<and> p' = High_cnode_ptr + 0x60 \<or>
           p = High_cnode_ptr + 0x60 \<and> p' = High_tcb_ptr + 0x20)"
-  supply option.case_cong[cong] if_cong[cong] s0_ptrs_aligned[simp]
+  supply [cong] = option.case_cong if_cong
+  supply [simp] = s0_ptrs_aligned
   apply (frule_tac x=p in map_to_ctes_kh0H_SomeD)
   apply (elim disjE, simp_all)
-          apply (frule_tac x=p' in map_to_ctes_kh0H_SomeD)
-          apply (elim disjE, simp_all add: sameRegionAs_def isCap_simps)[1]
-            apply (clarsimp simp: kh0H_all_obj_def' s0_ptr_defs split: if_split_asm)
-           apply (clarsimp simp: kh0H_all_obj_def' s0_ptr_defs split: if_split_asm)
-          apply (clarsimp simp: to_bl_use_of_bl the_nat_to_bl_simps kh0H_all_obj_def' ucast_shiftr_2
-                         split: if_split_asm)
+         (* p = Low_tcb_ptr (+ x) and p = High_tcb_ptr (+ x) cases *)
          apply ((frule_tac x=p' in map_to_ctes_kh0H_SomeD,
-                (elim disjE, simp_all add: sameRegionAs_def RISCV64_H.sameRegionAs_def isCap_simps)[1],
-                ((clarsimp simp: sameRegionAs_def RISCV64_H.sameRegionAs_def isCap_simps to_bl_use_of_bl
+                (elim disjE, simp_all add: sameRegionAs_def RISCV64_H.sameRegionAs_def isCap_simps)[1];
+                (clarsimp simp: sameRegionAs_def RISCV64_H.sameRegionAs_def isCap_simps to_bl_use_of_bl
                                  the_nat_to_bl_simps kh0H_all_obj_def' ucast_shiftr_2 ucast_shiftr_3
-                          split: if_split_asm)+)[3])+)[5]
+                                 cte_level_bits_def
+                          split: if_split_asm))+)[6]
+     (* init_irq_node *)
+     apply (clarsimp simp: kh0H_all_obj_def')
+    (* Silc_cnode_ptr *)
     apply (clarsimp simp: kh0H_all_obj_def' split: if_split_asm)
       apply (frule_tac x=p' in map_to_ctes_kh0H_SomeD)
       apply (elim disjE, simp_all add: sameRegionAs_def isCap_simps)[1]
-        apply (clarsimp simp: kh0H_all_obj_def' to_bl_use_of_bl the_nat_to_bl_simps
+         apply (clarsimp simp: kh0H_all_obj_def')
+        apply (clarsimp simp: kh0H_all_obj_def' to_bl_use_of_bl the_nat_to_bl_simps cte_level_bits_def
                        split: if_split_asm)
         apply (drule(2) ucast_shiftr_13E; clarsimp)
         apply (drule(2) ucast_shiftr_13E; clarsimp)
-       apply (clarsimp simp: kh0H_all_obj_def' to_bl_use_of_bl the_nat_to_bl_simps ucast_shiftr_13E
+       apply (clarsimp simp: kh0H_all_obj_def' to_bl_use_of_bl the_nat_to_bl_simps ucast_shiftr_13E cte_level_bits_def
                       split: if_split_asm)
-      apply (clarsimp simp: kh0H_all_obj_def' to_bl_use_of_bl the_nat_to_bl_simps ucast_shiftr_13E
+      apply (clarsimp simp: kh0H_all_obj_def' to_bl_use_of_bl the_nat_to_bl_simps ucast_shiftr_13E cte_level_bits_def
                      split: if_split_asm)
      apply (frule_tac x=p' in map_to_ctes_kh0H_SomeD)
      apply (elim disjE, simp_all add: sameRegionAs_def RISCV64_H.sameRegionAs_def isCap_simps
                                split: if_split_asm)[1]
-       apply (clarsimp simp: kh0H_all_obj_def' to_bl_use_of_bl the_nat_to_bl_simps split: if_split_asm)
+        apply (clarsimp simp: kh0H_all_obj_def')
+       apply (clarsimp simp: kh0H_all_obj_def' to_bl_use_of_bl the_nat_to_bl_simps cte_level_bits_def split: if_split_asm)
        apply (drule(2) ucast_shiftr_5; clarsimp)
        apply (drule(2) ucast_shiftr_5; clarsimp)
-      apply (clarsimp simp: kh0H_all_obj_def' to_bl_use_of_bl the_nat_to_bl_simps split: if_split_asm)
+      apply (clarsimp simp: kh0H_all_obj_def' to_bl_use_of_bl the_nat_to_bl_simps cte_level_bits_def split: if_split_asm)
       apply (drule(2) ucast_shiftr_5; clarsimp)
       apply (drule(2) ucast_shiftr_5; clarsimp)
-     apply (clarsimp simp: kh0H_all_obj_def' to_bl_use_of_bl the_nat_to_bl_simps split: if_split_asm)
+     apply (clarsimp simp: kh0H_all_obj_def' to_bl_use_of_bl the_nat_to_bl_simps cte_level_bits_def split: if_split_asm)
      apply (drule(2) ucast_shiftr_5; clarsimp)
      apply (drule(2) ucast_shiftr_5; clarsimp)
     apply (frule_tac x=p' in map_to_ctes_kh0H_SomeD)
     apply (elim disjE, simp_all add: sameRegionAs_def RISCV64_H.sameRegionAs_def isCap_simps
                               split: if_split_asm)[1]
-      apply (clarsimp simp: kh0H_all_obj_def' to_bl_use_of_bl the_nat_to_bl_simps split: if_split_asm)
+       apply (clarsimp simp: kh0H_all_obj_def')
+      apply (clarsimp simp: kh0H_all_obj_def' to_bl_use_of_bl the_nat_to_bl_simps cte_level_bits_def split: if_split_asm)
       apply (drule(2) ucast_shiftr_2; clarsimp)
       apply (drule(2) ucast_shiftr_2; clarsimp)
      apply (clarsimp simp: kh0H_all_obj_def' to_bl_use_of_bl the_nat_to_bl_simps split: if_split_asm)
     apply (clarsimp simp: kh0H_all_obj_def' to_bl_use_of_bl the_nat_to_bl_simps split: if_split_asm)
+   (* High_cnode_ptr *)
    apply (clarsimp simp: kh0H_all_obj_def' split: if_split_asm)
          apply (frule_tac x=p' in map_to_ctes_kh0H_SomeD)
          apply (elim disjE, simp_all add: sameRegionAs_def isCap_simps)[1]
+            apply (clarsimp simp: kh0H_all_obj_def')
            apply (clarsimp simp: kh0H_all_obj_def' to_bl_use_of_bl the_nat_to_bl_simps ucast_shiftr_13E
+                                 cte_level_bits_def
                           split: if_split_asm)
-          apply (clarsimp simp: kh0H_all_obj_def' to_bl_use_of_bl the_nat_to_bl_simps split: if_split_asm)
+          apply (clarsimp simp: kh0H_all_obj_def' to_bl_use_of_bl the_nat_to_bl_simps
+                                cte_level_bits_def
+                          split: if_split_asm)
           apply (drule(2) ucast_shiftr_13E; clarsimp)
           apply (drule(2) ucast_shiftr_13E; clarsimp)
          apply (clarsimp simp: kh0H_all_obj_def' to_bl_use_of_bl the_nat_to_bl_simps ucast_shiftr_13E
+                               cte_level_bits_def
                         split: if_split_asm)
         apply (frule_tac x=p' in map_to_ctes_kh0H_SomeD)
         apply (elim disjE, simp_all add: sameRegionAs_def RISCV64_H.sameRegionAs_def isCap_simps
                                   split: if_split_asm)[1]
+           apply (clarsimp simp: kh0H_all_obj_def')
           apply (clarsimp simp: kh0H_all_obj_def' to_bl_use_of_bl the_nat_to_bl_simps ucast_shiftr_3
+                                cte_level_bits_def
                          split: if_split_asm)
          apply (clarsimp simp: kh0H_all_obj_def' to_bl_use_of_bl the_nat_to_bl_simps
+                               cte_level_bits_def
                         split: if_split_asm)
          apply (drule(2) ucast_shiftr_6; clarsimp)
          apply (drule(2) ucast_shiftr_6; clarsimp)
@@ -2899,128 +2756,164 @@ lemma sameRegionAs_s0H:
        apply (frule_tac x=p' in map_to_ctes_kh0H_SomeD)
        apply (elim disjE, simp_all add: sameRegionAs_def RISCV64_H.sameRegionAs_def isCap_simps
                                  split: if_split_asm)[1]
+          apply (clarsimp simp: kh0H_all_obj_def')
          apply (clarsimp simp: kh0H_all_obj_def' to_bl_use_of_bl the_nat_to_bl_simps ucast_shiftr_3
+                               cte_level_bits_def
                         split: if_split_asm)
          apply (drule(2) ucast_shiftr_5; clarsimp)
          apply (drule(2) ucast_shiftr_5; clarsimp)
-        apply (clarsimp simp: kh0H_all_obj_def' to_bl_use_of_bl the_nat_to_bl_simps split: if_split_asm)
+        apply (clarsimp simp: kh0H_all_obj_def' to_bl_use_of_bl the_nat_to_bl_simps
+                              cte_level_bits_def
+                        split: if_split_asm)
         apply (drule(2) ucast_shiftr_5; clarsimp)
         apply (drule(2) ucast_shiftr_5; clarsimp)
-       apply (clarsimp simp: kh0H_all_obj_def' to_bl_use_of_bl the_nat_to_bl_simps split: if_split_asm)
+       apply (clarsimp simp: kh0H_all_obj_def' to_bl_use_of_bl the_nat_to_bl_simps
+                             cte_level_bits_def
+                       split: if_split_asm)
        apply (drule(2) ucast_shiftr_5; clarsimp)
        apply (drule(2) ucast_shiftr_5; clarsimp)
       apply (frule_tac x=p' in map_to_ctes_kh0H_SomeD)
       apply (elim disjE, simp_all add: sameRegionAs_def RISCV64_H.sameRegionAs_def isCap_simps
                                 split: if_split_asm)[1]
+         apply (clarsimp simp: kh0H_all_obj_def')
         apply (clarsimp simp: kh0H_all_obj_def' to_bl_use_of_bl the_nat_to_bl_simps ucast_shiftr_3
                        split: if_split_asm)
-       apply (clarsimp simp: kh0H_all_obj_def' to_bl_use_of_bl the_nat_to_bl_simps split: if_split_asm)
+       apply (clarsimp simp: kh0H_all_obj_def' to_bl_use_of_bl the_nat_to_bl_simps cte_level_bits_def
+                       split: if_split_asm)
        apply (drule(2) ucast_shiftr_4; clarsimp)
        apply (drule(2) ucast_shiftr_4; clarsimp)
       apply (clarsimp simp: kh0H_all_obj_def' to_bl_use_of_bl the_nat_to_bl_simps split: if_split_asm)
      apply (frule_tac x=p' in map_to_ctes_kh0H_SomeD)
      apply (elim disjE, simp_all add: sameRegionAs_def RISCV64_H.sameRegionAs_def isCap_simps
                                split: if_split_asm)[1]
+         apply (clarsimp simp: kh0H_all_obj_def' to_bl_use_of_bl the_nat_to_bl_simps ucast_shiftr_3
+                               cte_level_bits_def)
         apply (clarsimp simp: kh0H_all_obj_def' to_bl_use_of_bl the_nat_to_bl_simps ucast_shiftr_3
+                              cte_level_bits_def
                        split: if_split_asm)
        apply (clarsimp simp: kh0H_all_obj_def' to_bl_use_of_bl the_nat_to_bl_simps split: if_split_asm)
-      apply (clarsimp simp: kh0H_all_obj_def' to_bl_use_of_bl the_nat_to_bl_simps split: if_split_asm)
+      apply (clarsimp simp: kh0H_all_obj_def' to_bl_use_of_bl the_nat_to_bl_simps cte_level_bits_def
+                      split: if_split_asm)
       apply (drule(2) ucast_shiftr_3; clarsimp)
       apply (drule(2) ucast_shiftr_3; clarsimp)
      apply (clarsimp simp: kh0H_all_obj_def' to_bl_use_of_bl the_nat_to_bl_simps split: if_split_asm)
     apply (frule_tac x=p' in map_to_ctes_kh0H_SomeD)
     apply (elim disjE, simp_all add: sameRegionAs_def RISCV64_H.sameRegionAs_def isCap_simps
                               split: if_split_asm)[1]
+        apply (clarsimp simp: kh0H_all_obj_def' to_bl_use_of_bl the_nat_to_bl_simps ucast_shiftr_3
+                              cte_level_bits_def
+                       split: if_split_asm)
+        apply (drule(2) ucast_shiftr_2; clarsimp)
+       apply (clarsimp simp: kh0H_all_obj_def' to_bl_use_of_bl the_nat_to_bl_simps split: if_split_asm)
+      apply (clarsimp simp: kh0H_all_obj_def' split: if_split_asm)
+     apply (clarsimp simp: kh0H_all_obj_def' to_bl_use_of_bl the_nat_to_bl_simps cte_level_bits_def
+                     split: if_split_asm)
+     apply (drule(2) ucast_shiftr_2; clarsimp)
+     apply (drule(2) ucast_shiftr_2; clarsimp)
+    apply (clarsimp simp: kh0H_all_obj_def' to_bl_use_of_bl the_nat_to_bl_simps split: if_split_asm)
+   apply (frule_tac x=p' in map_to_ctes_kh0H_SomeD)
+   apply (elim disjE, simp_all add: sameRegionAs_def RISCV64_H.sameRegionAs_def isCap_simps
+                             split: if_split_asm)[1]
+      apply (clarsimp simp: kh0H_all_obj_def')
+     apply (clarsimp simp: kh0H_all_obj_def' to_bl_use_of_bl the_nat_to_bl_simps ucast_shiftr_3
+                           cte_level_bits_def
+                    split: if_split_asm)
+    apply (clarsimp simp: kh0H_all_obj_def' to_bl_use_of_bl the_nat_to_bl_simps cte_level_bits_def
+                    split: if_split_asm)
+    apply (drule(2) ucast_shiftr_1; clarsimp)
+    apply (drule(2) ucast_shiftr_1; clarsimp)
+   apply (clarsimp simp: kh0H_all_obj_def' to_bl_use_of_bl the_nat_to_bl_simps split: if_split_asm)
+  (* Low_cnode_ptr *)
+  apply (clarsimp simp: kh0H_all_obj_def' split: if_split_asm)
+        apply (frule_tac x=p' in map_to_ctes_kh0H_SomeD)
+        apply (elim disjE, simp_all add: sameRegionAs_def isCap_simps)[1]
+           apply (clarsimp simp: kh0H_all_obj_def')
+          apply (clarsimp simp: kh0H_all_obj_def' to_bl_use_of_bl the_nat_to_bl_simps cte_level_bits_def split: if_split_asm)
+          apply (drule(2) ucast_shiftr_13E; clarsimp)
+          apply (drule(2) ucast_shiftr_13E; clarsimp)
+         apply (clarsimp simp: kh0H_all_obj_def' to_bl_use_of_bl the_nat_to_bl_simps ucast_shiftr_13E
+                               cte_level_bits_def
+                        split: if_split_asm)
+        apply (clarsimp simp: kh0H_all_obj_def' to_bl_use_of_bl the_nat_to_bl_simps ucast_shiftr_13E
+                              cte_level_bits_def
+                       split: if_split_asm)
+        apply (drule(2) ucast_shiftr_13E; clarsimp)
+        apply (drule(2) ucast_shiftr_13E; clarsimp)
+       apply (frule_tac x=p' in map_to_ctes_kh0H_SomeD)
+       apply (elim disjE, simp_all add: sameRegionAs_def RISCV64_H.sameRegionAs_def isCap_simps
+                                 split: if_split_asm)[1]
+          apply (clarsimp simp: kh0H_all_obj_def')
+         apply (clarsimp simp: kh0H_all_obj_def' to_bl_use_of_bl the_nat_to_bl_simps ucast_shiftr_3
+                        split: if_split_asm)
+        apply (clarsimp simp: kh0H_all_obj_def' to_bl_use_of_bl the_nat_to_bl_simps split: if_split_asm)
+       apply (clarsimp simp: kh0H_all_obj_def' to_bl_use_of_bl the_nat_to_bl_simps cte_level_bits_def
+                       split: if_split_asm)
+       apply (drule(2) ucast_shiftr_6; clarsimp)
+       apply (drule(2) ucast_shiftr_6; clarsimp)
+      apply (frule_tac x=p' in map_to_ctes_kh0H_SomeD)
+      apply (elim disjE, simp_all add: sameRegionAs_def RISCV64_H.sameRegionAs_def isCap_simps
+                                split: if_split_asm)[1]
+         apply (clarsimp simp: kh0H_all_obj_def')
+        apply (clarsimp simp: kh0H_all_obj_def' to_bl_use_of_bl the_nat_to_bl_simps ucast_shiftr_3
+                              cte_level_bits_def
+                       split: if_split_asm)
+        apply (drule(2) ucast_shiftr_5; clarsimp)
+        apply (drule(2) ucast_shiftr_5; clarsimp)
+       apply (clarsimp simp: kh0H_all_obj_def' to_bl_use_of_bl the_nat_to_bl_simps cte_level_bits_def
+                      split: if_split_asm)
+       apply (drule(2) ucast_shiftr_5; clarsimp)
+       apply (drule(2) ucast_shiftr_5; clarsimp)
+      apply (clarsimp simp: kh0H_all_obj_def' to_bl_use_of_bl the_nat_to_bl_simps cte_level_bits_def
+                     split: if_split_asm)
+      apply (drule(2) ucast_shiftr_5; clarsimp)
+      apply (drule(2) ucast_shiftr_5; clarsimp)
+     apply (frule_tac x=p' in map_to_ctes_kh0H_SomeD)
+     apply (elim disjE, simp_all add: sameRegionAs_def RISCV64_H.sameRegionAs_def isCap_simps
+                               split: if_split_asm)[1]
+        apply (clarsimp simp: kh0H_all_obj_def')
        apply (clarsimp simp: kh0H_all_obj_def' to_bl_use_of_bl the_nat_to_bl_simps ucast_shiftr_3
+                      split: if_split_asm)
+      apply (clarsimp simp: kh0H_all_obj_def' to_bl_use_of_bl the_nat_to_bl_simps split: if_split_asm)
+     apply (clarsimp simp: kh0H_all_obj_def' to_bl_use_of_bl the_nat_to_bl_simps cte_level_bits_def
+                     split: if_split_asm)
+     apply (drule(2) ucast_shiftr_4; clarsimp)
+     apply (drule(2) ucast_shiftr_4; clarsimp)
+    apply (frule_tac x=p' in map_to_ctes_kh0H_SomeD)
+    apply (elim disjE, simp_all add: sameRegionAs_def RISCV64_H.sameRegionAs_def isCap_simps
+                              split: if_split_asm)[1]
+        apply (clarsimp simp: kh0H_all_obj_def' to_bl_use_of_bl the_nat_to_bl_simps ucast_shiftr_3
+                              cte_level_bits_def
+                       split: if_split_asm)
+       apply (clarsimp simp: kh0H_all_obj_def' to_bl_use_of_bl the_nat_to_bl_simps split: if_split_asm)
+      apply (clarsimp simp: kh0H_all_obj_def' to_bl_use_of_bl the_nat_to_bl_simps split: if_split_asm)
+     apply (clarsimp simp: kh0H_all_obj_def' to_bl_use_of_bl the_nat_to_bl_simps split: if_split_asm)
+    apply (clarsimp simp: kh0H_all_obj_def' to_bl_use_of_bl the_nat_to_bl_simps cte_level_bits_def
+                    split: if_split_asm)
+    apply (drule(2) ucast_shiftr_3; clarsimp)
+    apply (drule(2) ucast_shiftr_3; clarsimp)
+   apply (frule_tac x=p' in map_to_ctes_kh0H_SomeD)
+   apply (elim disjE, simp_all add: sameRegionAs_def RISCV64_H.sameRegionAs_def isCap_simps
+                             split: if_split_asm)[1]
+       apply (clarsimp simp: kh0H_all_obj_def' to_bl_use_of_bl the_nat_to_bl_simps ucast_shiftr_3
+                             cte_level_bits_def
                       split: if_split_asm)
        apply (drule(2) ucast_shiftr_2; clarsimp)
       apply (clarsimp simp: kh0H_all_obj_def' to_bl_use_of_bl the_nat_to_bl_simps split: if_split_asm)
      apply (clarsimp simp: kh0H_all_obj_def' to_bl_use_of_bl the_nat_to_bl_simps split: if_split_asm)
-     apply (drule(2) ucast_shiftr_2; clarsimp)
-     apply (drule(2) ucast_shiftr_2; clarsimp)
     apply (clarsimp simp: kh0H_all_obj_def' to_bl_use_of_bl the_nat_to_bl_simps split: if_split_asm)
-   apply (frule_tac x=p' in map_to_ctes_kh0H_SomeD)
-   apply (elim disjE, simp_all add: sameRegionAs_def RISCV64_H.sameRegionAs_def isCap_simps
-                             split: if_split_asm)[1]
-     apply (clarsimp simp: kh0H_all_obj_def' to_bl_use_of_bl the_nat_to_bl_simps ucast_shiftr_3
-                    split: if_split_asm)
-    apply (clarsimp simp: kh0H_all_obj_def' to_bl_use_of_bl the_nat_to_bl_simps split: if_split_asm)
-    apply (drule(2) ucast_shiftr_1; clarsimp)
-    apply (drule(2) ucast_shiftr_1; clarsimp)
-   apply (clarsimp simp: kh0H_all_obj_def' to_bl_use_of_bl the_nat_to_bl_simps split: if_split_asm)
-  apply (clarsimp simp: kh0H_all_obj_def' split: if_split_asm)
-        apply (frule_tac x=p' in map_to_ctes_kh0H_SomeD)
-        apply (elim disjE, simp_all add: sameRegionAs_def isCap_simps)[1]
-          apply (clarsimp simp: kh0H_all_obj_def' to_bl_use_of_bl the_nat_to_bl_simps ucast_shiftr_13E
-                         split: if_split_asm)
-         apply (clarsimp simp: kh0H_all_obj_def' to_bl_use_of_bl the_nat_to_bl_simps split: if_split_asm)
-         apply (drule(2) ucast_shiftr_13E; clarsimp)
-         apply (drule(2) ucast_shiftr_13E; clarsimp)
-        apply (clarsimp simp: kh0H_all_obj_def' to_bl_use_of_bl the_nat_to_bl_simps ucast_shiftr_13E
-                       split: if_split_asm)
-        apply (drule(2) ucast_shiftr_13E; clarsimp)
-        apply (drule(2) ucast_shiftr_13E; clarsimp)
-       apply (frule_tac x=p' in map_to_ctes_kh0H_SomeD)
-       apply (elim disjE, simp_all add: sameRegionAs_def RISCV64_H.sameRegionAs_def isCap_simps
-                                 split: if_split_asm)[1]
-         apply (clarsimp simp: kh0H_all_obj_def' to_bl_use_of_bl the_nat_to_bl_simps ucast_shiftr_3
-                        split: if_split_asm)
-        apply (clarsimp simp: kh0H_all_obj_def' to_bl_use_of_bl the_nat_to_bl_simps split: if_split_asm)
-       apply (clarsimp simp: kh0H_all_obj_def' to_bl_use_of_bl the_nat_to_bl_simps split: if_split_asm)
-       apply (drule(2) ucast_shiftr_6; clarsimp)
-       apply (drule(2) ucast_shiftr_6; clarsimp)
-      apply (frule_tac x=p' in map_to_ctes_kh0H_SomeD)
-      apply (elim disjE, simp_all add: sameRegionAs_def RISCV64_H.sameRegionAs_def isCap_simps
-                                split: if_split_asm)[1]
-        apply (clarsimp simp: kh0H_all_obj_def' to_bl_use_of_bl the_nat_to_bl_simps ucast_shiftr_3
-                       split: if_split_asm)
-        apply (drule(2) ucast_shiftr_5; clarsimp)
-        apply (drule(2) ucast_shiftr_5; clarsimp)
-       apply (clarsimp simp: kh0H_all_obj_def' to_bl_use_of_bl the_nat_to_bl_simps
-                      split: if_split_asm)
-       apply (drule(2) ucast_shiftr_5; clarsimp)
-       apply (drule(2) ucast_shiftr_5; clarsimp)
-      apply (clarsimp simp: kh0H_all_obj_def' to_bl_use_of_bl the_nat_to_bl_simps
-                     split: if_split_asm)
-      apply (drule(2) ucast_shiftr_5; clarsimp)
-      apply (drule(2) ucast_shiftr_5; clarsimp)
-     apply (frule_tac x=p' in map_to_ctes_kh0H_SomeD)
-     apply (elim disjE, simp_all add: sameRegionAs_def RISCV64_H.sameRegionAs_def isCap_simps
-                               split: if_split_asm)[1]
-       apply (clarsimp simp: kh0H_all_obj_def' to_bl_use_of_bl the_nat_to_bl_simps ucast_shiftr_3
-                      split: if_split_asm)
-      apply (clarsimp simp: kh0H_all_obj_def' to_bl_use_of_bl the_nat_to_bl_simps split: if_split_asm)
-     apply (clarsimp simp: kh0H_all_obj_def' to_bl_use_of_bl the_nat_to_bl_simps split: if_split_asm)
-     apply (drule(2) ucast_shiftr_4; clarsimp)
-     apply (drule(2) ucast_shiftr_4; clarsimp)
-    apply (frule_tac x=p' in map_to_ctes_kh0H_SomeD)
-    apply (elim disjE, simp_all add: sameRegionAs_def RISCV64_H.sameRegionAs_def isCap_simps
-                              split: if_split_asm)[1]
-       apply (clarsimp simp: kh0H_all_obj_def' to_bl_use_of_bl the_nat_to_bl_simps ucast_shiftr_3
-                      split: if_split_asm)
-      apply (clarsimp simp: kh0H_all_obj_def' to_bl_use_of_bl the_nat_to_bl_simps split: if_split_asm)
-     apply (clarsimp simp: kh0H_all_obj_def' to_bl_use_of_bl the_nat_to_bl_simps split: if_split_asm)
-    apply (clarsimp simp: kh0H_all_obj_def' to_bl_use_of_bl the_nat_to_bl_simps split: if_split_asm)
-    apply (drule(2) ucast_shiftr_3; clarsimp)
-    apply (drule(2) ucast_shiftr_3; clarsimp)
-   apply (frule_tac x=p' in map_to_ctes_kh0H_SomeD)
-   apply (elim disjE, simp_all add: sameRegionAs_def RISCV64_H.sameRegionAs_def isCap_simps
-                             split: if_split_asm)[1]
-      apply (clarsimp simp: kh0H_all_obj_def' to_bl_use_of_bl the_nat_to_bl_simps ucast_shiftr_3
-                     split: if_split_asm)
-      apply (drule(2) ucast_shiftr_2; clarsimp)
-     apply (clarsimp simp: kh0H_all_obj_def' to_bl_use_of_bl the_nat_to_bl_simps split: if_split_asm)
-    apply (clarsimp simp: kh0H_all_obj_def' to_bl_use_of_bl the_nat_to_bl_simps split: if_split_asm)
-   apply (clarsimp simp: kh0H_all_obj_def' to_bl_use_of_bl the_nat_to_bl_simps split: if_split_asm)
+   apply (clarsimp simp: kh0H_all_obj_def' to_bl_use_of_bl the_nat_to_bl_simps cte_level_bits_def
+                   split: if_split_asm)
    apply (drule(2) ucast_shiftr_2; clarsimp)
    apply (drule(2) ucast_shiftr_2; clarsimp)
   apply (frule_tac x=p' in map_to_ctes_kh0H_SomeD)
   apply (elim disjE, simp_all add: sameRegionAs_def RISCV64_H.sameRegionAs_def isCap_simps
                             split: if_split_asm)[1]
-    apply (clarsimp simp: kh0H_all_obj_def' to_bl_use_of_bl the_nat_to_bl_simps ucast_shiftr_3
-                   split: if_split_asm)
+     apply (clarsimp simp: kh0H_all_obj_def' to_bl_use_of_bl the_nat_to_bl_simps ucast_shiftr_3
+                    split: if_split_asm)
+    apply (clarsimp simp: kh0H_all_obj_def' to_bl_use_of_bl the_nat_to_bl_simps split: if_split_asm)
    apply (clarsimp simp: kh0H_all_obj_def' to_bl_use_of_bl the_nat_to_bl_simps split: if_split_asm)
-  apply (clarsimp simp: kh0H_all_obj_def' to_bl_use_of_bl the_nat_to_bl_simps split: if_split_asm)
+  apply (clarsimp simp: kh0H_all_obj_def' to_bl_use_of_bl the_nat_to_bl_simps cte_level_bits_def
+                  split: if_split_asm)
   apply (drule(2) ucast_shiftr_1; clarsimp)
   apply (drule(2) ucast_shiftr_1; clarsimp)
   done
@@ -3039,7 +2932,7 @@ lemma s0H_valid_pspace':
   assumes "1 \<le> maxDomain"
   shows "valid_pspace' s0H_internal"
   using assms
-  supply option.case_cong[cong] if_cong[cong]
+  supply option.case_cong[cong] if_cong[cong] cte_level_bits_def[simp]
   apply (clarsimp simp: valid_pspace'_def s0H_pspace_distinct' s0H_valid_objs')
   apply (intro conjI)
       apply (clarsimp simp: pspace_aligned'_def)
@@ -3091,7 +2984,8 @@ lemma s0H_valid_pspace':
                            apply ((rule r_r_into_trancl[OF next_fold next_fold], simp+)+)[2]
                          apply ((erule r_into_trancl[OF next_fold], clarsimp)+)[3]
                       apply ((rule r_r_into_trancl[OF next_fold next_fold], simp+)+)[2]
-                    apply ((erule r_into_trancl[OF next_fold], clarsimp)+)[5]
+                    apply ((erule r_into_trancl[OF next_fold], clarsimp)+)[4]
+                apply (simp add: irq_cte_def)
                apply (clarsimp simp: kh0H_all_obj_def Silc_cte_cte_def cnode_offs_range_def
                               split: if_split_asm)
                   apply ((rule r_r_into_trancl[OF next_fold next_fold], simp+)+)[2]
@@ -3135,7 +3029,7 @@ lemma s0H_valid_pspace':
                                         split: if_split_asm)+)[1]
            apply (clarsimp simp: caps_contained'_def)
            apply (drule_tac x=p in map_to_ctes_kh0H_SomeD)
-           apply (elim disjE, simp_all)[1]
+           apply (elim disjE, simp_all add: irq_cte_def)[1]
              apply (clarsimp simp: Silc_cte_cte_def kh0H_all_obj_def split: if_split_asm)
             apply (clarsimp simp: High_cte_cte_def kh0H_all_obj_def split: if_split_asm)
            apply (clarsimp simp: Low_cte_cte_def kh0H_all_obj_def split: if_split_asm)
@@ -3310,7 +3204,9 @@ lemma s0H_invs:
       apply (rule_tac x="High_cnode_ptr + 0x20" in exI)
       apply (clarsimp simp: kh0H_all_obj_def' image_def)
      apply (rule_tac x="Silc_cnode_ptr + 0x40" in exI)
-     apply (clarsimp simp: kh0H_all_obj_def' image_def to_bl_use_of_bl the_nat_to_bl_simps split: if_split_asm)
+     apply (clarsimp simp: kh0H_all_obj_def' image_def to_bl_use_of_bl the_nat_to_bl_simps
+                           cte_level_bits_def
+                     split: if_split_asm)
        apply (drule(2) ucast_shiftr_13E, rule s0_ptrs_aligned, simp)
        apply (rule_tac x="(0x27C0 >> 5)" in bexI)
         apply simp
@@ -3324,7 +3220,9 @@ lemma s0H_invs:
       apply simp
      apply (simp add: mask_def)
     apply (rule_tac x="High_cnode_ptr + 0x40" in exI)
-    apply (clarsimp simp: kh0H_all_obj_def' image_def to_bl_use_of_bl the_nat_to_bl_simps split: if_split_asm)
+    apply (clarsimp simp: kh0H_all_obj_def' image_def to_bl_use_of_bl the_nat_to_bl_simps
+                          cte_level_bits_def
+                    split: if_split_asm)
           apply (drule(2) ucast_shiftr_13E, rule s0_ptrs_aligned, simp)
           apply (rule_tac x="0x13E" in bexI)
            apply simp
@@ -3354,7 +3252,9 @@ lemma s0H_invs:
      apply simp
     apply (simp add: mask_def)
    apply (rule_tac x="Low_cnode_ptr + 0x40" in exI)
-   apply (clarsimp simp: kh0H_all_obj_def' image_def to_bl_use_of_bl the_nat_to_bl_simps split: if_split_asm)
+   apply (clarsimp simp: kh0H_all_obj_def' image_def to_bl_use_of_bl the_nat_to_bl_simps
+                         cte_level_bits_def
+                   split: if_split_asm)
          apply (drule(2) ucast_shiftr_13E, rule s0_ptrs_aligned, simp)
          apply (rule_tac x="0x13E" in bexI)
           apply simp
@@ -3399,13 +3299,14 @@ lemma s0H_invs:
    apply (rule conjI)
     apply (clarsimp simp: s0H_internal_def is_aligned_def s0_ptr_defs word_size)
    apply (clarsimp simp: obj_at'_def objBitsKO_def s0H_internal_def
+                         kh0H_simps(1)[unfolded cte_level_bits_def]
                          shiftl_t2n[where n=4, simplified, symmetric])
    apply (rule conjI)
     apply (rule is_aligned_add)
      apply (simp add: is_aligned_def s0_ptr_defs)
     apply (rule is_aligned_shift)
    apply (rule pspace_distinctD''[OF _ s0H_pspace_distinct', simplified s0H_internal_def])
-   apply (simp add: objBitsKO_def)
+   apply (simp add: objBitsKO_def kh0H_simps(1)[unfolded cte_level_bits_def])
   apply (rule conjI)
    apply (clarsimp simp: valid_irq_handlers'_def cteCaps_of_def ran_def)
    apply (drule_tac map_to_ctes_kh0H_SomeD)
@@ -3416,13 +3317,14 @@ lemma s0H_invs:
   apply (rule conjI)
    apply (clarsimp simp: valid_machine_state'_def s0H_internal_def machine_state0_def)
   apply (rule conjI)
-   apply (clarsimp simp: irqs_masked'_def s0H_internal_def maxIRQ_def timer_irq_def irqInvalid_def)
+   using timer_irq_le_maxIRQ
+   apply (fastforce simp: irqs_masked'_def s0H_internal_def maxIRQ_def )
   apply (rule conjI)
-   apply (clarsimp simp: sym_heap_def opt_map_def projectKOs split: option.splits)
+   apply (clarsimp simp: sym_heap_def opt_map_def split: option.splits)
    using kh0H_dom_tcb
    apply (fastforce simp: kh0H_obj_def)
   apply (rule conjI)
-   apply (clarsimp simp: valid_sched_pointers_def opt_map_def projectKOs split: option.splits)
+   apply (clarsimp simp: valid_sched_pointers_def opt_map_def split: option.splits)
    using kh0H_dom_tcb
    apply (fastforce simp: kh0H_obj_def)
   apply (rule conjI)
@@ -3449,9 +3351,13 @@ lemma s0H_invs:
   apply (simp add: objBitsKO_def)
   done
 
+lemma well_formed_cnode_n_0[simp]:
+  "well_formed_cnode_n 0 [[] \<mapsto> cap]"
+  by (simp add: well_formed_cnode_n_def)
+
 lemma kh0_pspace_dom:
   "pspace_dom kh0 = {idle_tcb_ptr, High_tcb_ptr, Low_tcb_ptr,
-                     High_pool_ptr, Low_pool_ptr, irq_cnode_ptr, ntfn_ptr} \<union>
+                     High_pool_ptr, Low_pool_ptr, ntfn_ptr} \<union>
                     irq_node_offs_range \<union>
                     page_offs_range shared_page_ptr_virt \<union>
                     cnode_offs_range Silc_cnode_ptr \<union>
@@ -3485,9 +3391,6 @@ lemma kh0_pspace_dom:
   apply (rule conjI)
    apply (rule_tac x=Low_pool_ptr in exI)
    apply (clarsimp simp: kh0_def kh0_obj_def s0_ptr_defs image_def)
-  apply (rule conjI)
-   apply (rule_tac x=irq_cnode_ptr in exI)
-   apply (clarsimp simp: kh0_def kh0_obj_def s0_ptr_defs image_def cte_map_def)
   apply (rule conjI)
    apply (rule_tac x=ntfn_ptr in exI)
    apply (clarsimp simp: kh0_def kh0_obj_def s0_ptr_defs image_def)
@@ -3598,50 +3501,48 @@ lemma s0_pspace_rel:
   apply clarsimp
   apply (drule kh0_SomeD)
   apply (elim disjE)
-                  apply (clarsimp simp: kh0_obj_def bit_simps dest!: less_0x200_exists_ucast)
-                 defer
-                 apply ((clarsimp simp: kh0_obj_def kh0H_obj_def bit_simps word_bits_def
-                                        fault_rel_optionation_def tcb_relation_cut_def
-                                        tcb_relation_def arch_tcb_relation_def the_nat_to_bl_simps
-                             split del: if_split)+)[3]
-              prefer 13
-              apply ((clarsimp simp: kh0_obj_def kh0H_all_obj_def bit_simps add.commute
-                                     pt_offs_max pt_offs_min pte_relation_def
-                          split del: if_split,
-                      clarsimp simp: s0_ptr_defs shared_page_ptr_phys_def addrFromPPtr_def pptrBaseOffset_def paddrBase_def
-                                     vmrights_map_def vm_read_only_def vm_read_write_def
-                                     kh0_obj_def kh0H_all_obj_def elf_index_value,
-                      (clarsimp simp: bit_simps mask_def)?)+)[5]
-         apply (clarsimp simp: kh0_obj_def kh0H_obj_def well_formed_cnode_n_def
-                               cte_relation_def cte_map_def bit_simps)
-        apply (clarsimp simp: kh0H_obj_def bit_simps ntfn_def other_obj_relation_def ntfn_relation_def)
-       defer
-       apply ((clarsimp simp: kh0_obj_def kh0H_obj_def other_obj_relation_def
-                              asid_pool_relation_def comp_def inv_into_def2 other_aobj_relation_def,
-               rule ext,
-               clarsimp simp: asid_low_bits_of_def asid_low_bits_def High_asid_def,
-               word_bitwise, fastforce)+)[2]
+                 apply (clarsimp simp: kh0_obj_def bit_simps dest!: less_0x200_exists_ucast)
+                defer
+                apply ((clarsimp simp: kh0_obj_def kh0H_obj_def bit_simps word_bits_def
+                                       fault_rel_optionation_def tcb_relation_cut_def
+                                       tcb_relation_def arch_tcb_relation_def the_nat_to_bl_simps
+                            split del: if_split)+)[3]
+             prefer 12
+             apply ((clarsimp simp: kh0_obj_def kh0H_all_obj_def bit_simps add.commute
+                                    pt_offs_max pt_offs_min pte_relation_def
+                         split del: if_split,
+                     clarsimp simp: s0_ptr_defs shared_page_ptr_phys_def addrFromPPtr_def pptrBaseOffset_def paddrBase_def
+                                    vmrights_map_def vm_read_only_def vm_read_write_def
+                                    kh0_obj_def kh0H_all_obj_def elf_index_value,
+                     (clarsimp simp: bit_simps mask_def)?)+)[5]
+         apply (clarsimp simp: kh0H_obj_def bit_simps ntfn_def other_obj_relation_def ntfn_relation_def)
+        defer
+        apply ((clarsimp simp: kh0_obj_def kh0H_obj_def other_obj_relation_def
+                               asid_pool_relation_def comp_def inv_into_def2 other_aobj_relation_def,
+                rule ext,
+                clarsimp simp: asid_low_bits_of_def asid_low_bits_def High_asid_def,
+                word_bitwise, fastforce)+)[2]
+      apply (clarsimp simp: kh0H_obj_def kh0_obj_def cte_relation_def cte_map_def')
+      apply (cut_tac dom_caps(2))[1]
+      apply (frule_tac m=High_caps in domI)
+      apply (cut_tac x=y in cnode_offs_in_range(2), simp)
+      apply (clarsimp simp: cnode_offs_range_def kh0H_all_obj_def High_caps_def cte_level_bits_def
+                            the_nat_to_bl_simps vmrights_map_def vm_read_only_def
+                     split: if_split_asm)
      apply (clarsimp simp: kh0H_obj_def kh0_obj_def cte_relation_def cte_map_def')
-     apply (cut_tac dom_caps(2))[1]
-     apply (frule_tac m=High_caps in domI)
-     apply (cut_tac x=y in cnode_offs_in_range(2), simp)
-     apply (clarsimp simp: cnode_offs_range_def kh0H_all_obj_def High_caps_def
-                           the_nat_to_bl_simps vmrights_map_def vm_read_only_def
+     apply (cut_tac dom_caps(3))[1]
+     apply (frule_tac m=Low_caps in domI)
+     apply (cut_tac x=y in cnode_offs_in_range(1), simp)
+     apply (clarsimp simp: cnode_offs_range_def kh0H_all_obj_def Low_caps_def cte_level_bits_def
+                           the_nat_to_bl_simps vmrights_map_def vm_read_write_def
                     split: if_split_asm)
-    apply (clarsimp simp: kh0H_obj_def kh0_obj_def cte_relation_def cte_map_def')
-    apply (cut_tac dom_caps(3))[1]
-    apply (frule_tac m=Low_caps in domI)
-    apply (cut_tac x=y in cnode_offs_in_range(1), simp)
-    apply (clarsimp simp: cnode_offs_range_def kh0H_all_obj_def Low_caps_def
-                          the_nat_to_bl_simps vmrights_map_def vm_read_write_def
-                   split: if_split_asm)
    apply (fastforce simp: kh0H_obj_def cte_map_def cte_relation_def well_formed_cnode_n_def
                     dest: irq_node_offs_range_correct split: if_split_asm)
   apply (clarsimp simp: kh0H_obj_def kh0_obj_def cte_relation_def cte_map_def')
   apply (cut_tac dom_caps(1))[1]
   apply (frule_tac m=Silc_caps in domI)
   apply (cut_tac x=y in cnode_offs_in_range(3), simp)
-  apply (clarsimp simp: cnode_offs_range_def kh0H_all_obj_def Silc_caps_def
+  apply (clarsimp simp: cnode_offs_range_def kh0H_all_obj_def Silc_caps_def cte_level_bits_def
                         the_nat_to_bl_simps vmrights_map_def vm_read_only_def
                  split: if_split_asm)
   done
@@ -3670,23 +3571,19 @@ lemma s0_srel:
                 apply (fastforce simp: kh0_def kh0_obj_def dest: kh0_SomeD)
                apply clarsimp
                apply (rule conjI)
-                apply clarsimp
-                apply (rule iffI)
-                 apply clarsimp
-                 apply (drule kh0_SomeD)
-                 apply (clarsimp simp: irq_node_offs_in_range)
-                apply (fastforce simp: kh0_def well_formed_cnode_n_def empty_cnode_def dom_def)
+                apply (fastforce simp: kh0_def well_formed_cnode_n_def empty_cnode_def dom_def
+                                       irq_node_offs_in_range
+                                 dest: kh0_SomeD)
                apply clarsimp
                apply (clarsimp simp: s0_ptr_defs)
                apply (subgoal_tac "a \<notin> irq_node_offs_range")
                 prefer 2
-                apply (clarsimp simp: irq_node_offs_range_def s0_ptr_defs)
-                apply (erule_tac x="ucast (a - 0xFFFFFFC000003000 >> 5)" in allE)
+                apply (clarsimp simp: irq_node_offs_range_def s0_ptr_defs irq_node_size_def irq_len_val cte_level_bits_def)
+                apply (erule_tac x="ucast (a - 0xFFFFFFC000030000 >> 5)" in allE)
                 apply (subst (asm) ucast_ucast_len)
                  apply (rule shiftr_less_t2n)
-                 apply (rule word_less_sub_right)
-                  apply (erule dual_order.strict_trans[rotated], clarsimp)
-                 apply clarsimp
+                 apply (simp add: is_aligned_def)
+                 apply unat_arith
                 apply (simp add: shiftr_shiftl1)
                 apply (subst(asm) is_aligned_neg_mask_eq)
                  apply (rule aligned_sub_aligned[where n=5])
@@ -3721,8 +3618,8 @@ lemma s0_srel:
                  apply clarsimp
                  apply (drule kh0_SomeD)
                  apply (clarsimp simp: s0_ptr_defs kh0_obj_def)
-                apply (fastforce simp: kh0_def kh0_obj_def dom_def s0_ptr_defs Silc_caps_def
-                                       well_formed_cnode_n_def empty_cnode_def)
+                apply (fastforce simp: s0_ptr_defs irq_node_offs_range_def cte_level_bits_def
+                                      is_aligned_def irq_node_size_def irq_len_val)
                apply clarsimp
                apply (drule kh0_SomeD)
                apply (clarsimp simp: s0_ptr_defs kh0_obj_def)
