proof/crefine/RISCV64/Finalise_C.thy
@@ -978,11 +978,11 @@ lemma unbindMaybeNotification_ccorres:
 (* TODO: move *)
 definition
   irq_opt_relation_def:
-  "irq_opt_relation (airq :: (6 word) option) (cirq :: machine_word) \<equiv>
+  "irq_opt_relation (airq :: irq option) (cirq :: machine_word) \<equiv>
        case airq of
          Some irq \<Rightarrow> (cirq = ucast irq \<and>
                       irq \<noteq> ucast irqInvalid \<and>
-                      ucast irq \<le> UCAST(32 signed \<rightarrow> 6) Kernel_C.maxIRQ)
+                      ucast irq \<le> UCAST(32 signed \<rightarrow> irq_len) Kernel_C.maxIRQ)
        | None \<Rightarrow> cirq = ucast irqInvalid"
 
 lemma finaliseCap_True_cases_ccorres:
@@ -1684,8 +1684,8 @@ lemma cteDeleteOne_ccorres:
 
 lemma getIRQSlot_ccorres_stuff:
   "\<lbrakk> (s, s') \<in> rf_sr \<rbrakk> \<Longrightarrow>
-   CTypesDefs.ptr_add intStateIRQNode_Ptr (uint (irq :: 6 word))
-     = Ptr (irq_node' s + 2 ^ cte_level_bits * ucast irq)"
+   CTypesDefs.ptr_add intStateIRQNode_Ptr (uint irq)
+   = Ptr (irq_node' s + 2 ^ cte_level_bits * ucast irq)" for irq :: irq
   apply (clarsimp simp add: rf_sr_def cstate_relation_def Let_def
                             cinterrupt_relation_def)
   apply (simp add: objBits_simps cte_level_bits_def
@@ -1723,10 +1723,9 @@ lemma deletingIRQHandler_ccorres:
   apply (clarsimp simp: cap_get_tag_isCap ghost_assertion_data_get_def
                         ghost_assertion_data_set_def)
   apply (simp add: cap_tag_defs)
-  apply (clarsimp simp: cte_wp_at_ctes_of Collect_const_mem
-                        irq_opt_relation_def Kernel_C.maxIRQ_def)
-  apply (drule word_le_nat_alt[THEN iffD1])
-  apply (clarsimp simp: uint_0_iff unat_gt_0 uint_up_ucast is_up)
+  using maxIRQ_less_2p_irqBits
+  apply (clarsimp simp: cte_wp_at_ctes_of Collect_const_mem word_le_nat_alt word_less_nat_alt
+                        irq_opt_relation_def Kernel_C_maxIRQ uint_0_iff unat_gt_0)
   done
 
 (* 6 = wordRadix,
@@ -1747,21 +1746,16 @@ lemma Zombie_new_spec:
   done
 
 lemma irq_opt_relation_Some_ucast:
-  "\<lbrakk> x && mask 6 = x; ucast x \<noteq> irqInvalid;
-    ucast x \<le> (scast Kernel_C.maxIRQ :: 6 word) \<or> x \<le> (scast Kernel_C.maxIRQ :: machine_word) \<rbrakk>
+  "\<lbrakk> x && mask irqBits = x; ucast x \<noteq> irqInvalid;
+    ucast x \<le> (scast Kernel_C.maxIRQ :: irq) \<or> x \<le> (scast Kernel_C.maxIRQ :: machine_word) \<rbrakk>
    \<Longrightarrow> irq_opt_relation (Some (ucast x)) x"
   unfolding irq_opt_relation_def
-  apply simp
-  using ucast_ucast_mask[where x=x and 'a=6, symmetric]
-  apply (simp add: irq_opt_relation_def)
-  apply (clarsimp simp: irqInvalid_def Kernel_C.maxIRQ_def)
-  apply (simp only: unat_arith_simps )
-  apply (clarsimp simp: word_le_nat_alt Kernel_C.maxIRQ_def)
-  done
+  using ucast_ucast_mask[where x=x and 'a=irq_len, unfolded LENGTH_irq_len_irqBits]
+  by (auto simp: Kernel_C_maxIRQ irq_machine_le_maxIRQ_irq)
 
 lemma ccap_relation_IRQHandler_mask:
   "\<lbrakk> ccap_relation acap ccap; isIRQHandlerCap acap \<rbrakk>
-    \<Longrightarrow> capIRQ_CL (cap_irq_handler_cap_lift ccap) && mask 6
+    \<Longrightarrow> capIRQ_CL (cap_irq_handler_cap_lift ccap) && mask irqBits
         = capIRQ_CL (cap_irq_handler_cap_lift ccap)"
   apply (simp only: cap_get_tag_isCap[symmetric])
   apply (drule ccap_relation_c_valid_cap)
@@ -2247,16 +2241,16 @@ lemma finaliseCap_ccorres:
     apply clarsimp
     apply (frule cap_get_tag_to_H, erule(1) cap_get_tag_isCap [THEN iffD2])
     apply (frule(1) ccap_relation_IRQHandler_mask)
-    apply (clarsimp simp: isCap_simps irqInvalid_def valid_cap'_def)
+    apply (clarsimp simp: isCap_simps valid_cap'_def)
     apply (rule irq_opt_relation_Some_ucast)
       apply fastforce
-     apply (simp add: irqInvalid_def)
-    apply (simp add: Kernel_C.maxIRQ_def maxIRQ_def)
+     apply simp
+    apply (simp add: Kernel_C_maxIRQ maxIRQ_def)
    apply fastforce
   apply clarsimp
   apply (frule cap_get_tag_to_H, erule(1) cap_get_tag_isCap [THEN iffD2])
   apply (frule(1) ccap_relation_IRQHandler_mask)
-  apply (clarsimp simp add:mask_eq_ucast_eq)
+  apply (clarsimp simp: ucast_ucast_mask simp flip: LENGTH_irq_len_irqBits)
   done
   end
 
